BF_CapFlow.thy
@@ -1,0 +1,68 @@
+
+theory BF_CapFlow
+imports Dynamic_model_v6 CapFlow_v6_0
+
+begin
+
+type_synonym systime_t = nat
+
+datatype
+  task_type =  TASK_TYPE_BEST_EFFORT
+              |TASK_TYPE_SOFT_REALTIME
+              |TASK_TYPE_HARD_REALTIME    
+
+datatype
+  sys_err =  SYS_ERR_OK
+              |SYS_ERR_CAP_NOT_FOUND
+              |SYS_ERR_LMP_TARGET_DISABLED   
+              |SYS_ERR_LMP_BUF_OVERFLOW
+
+record dcb = disabled :: bool
+             is_vm_guest :: bool
+             domain_id_dcb :: domain_id
+             type :: task_type
+             wakeup_time :: systime_t
+             release_time :: systime_t
+             etime :: systime_t
+             last_dispatch :: systime_t
+             wcet :: systime_t
+             period :: systime_t
+             deadline :: systime_t
+             weight :: nat
+
+
+record StateR = State + 
+                dispatchers :: "domain_id \<Rightarrow> dcb"
+
+definition abstract_state :: "StateR \<Rightarrow> State" ("\<Up>_" [50])        
+
+
+  where "abstract_state r = \<lparr>caps = caps r,
+                            e_msgs = e_msgs r,
+                            e_buf_size = e_buf_size r,
+                            domain_endpoint = domain_endpoint r
+                           \<rparr>"
+
+definition abstract_state_rev :: "StateR \<Rightarrow> State \<Rightarrow> StateR" ("_\<Down>_" [50])
+  where "abstract_state_rev r' r = r'\<lparr>caps := caps r,
+                            e_msgs := e_msgs r,
+                            e_buf_size := e_buf_size r,
+                            domain_endpoint := domain_endpoint r\<rparr>"
+
+definition sys_dispatcher_properties :: "StateR \<Rightarrow> domain_id \<Rightarrow> systime_t \<Rightarrow> (StateR \<times> bool )" where
+  "sys_dispatcher_properties sr did p_type p_deadline p_wcet p_period p_release p_weight p_wcet \<equiv>   
+                  let
+                    new_dispatchers = dispatchers sr;
+                    t_dcb = new_dispatchers did;
+                    new_dcb = t_dcb
+                                \<lparr> wcet := p_wcet,
+                                  is_vm_guest := is_vm_guest t_dcb,
+                                  domain_id_dcb := domain_id_dcb t_dcb,
+                                  wakeup_time := wakeup_time t_dcb,
+                                  release_time := release_time t_dcb\<rparr>
+                  in
+                    (sr\<lparr>
+                      dispatchers := new_dispatchers(did := new_dcb)
+                      \<rparr>, True)"
+
+end
