SK_L2Spec.thy
@@ -1,0 +1,2083 @@
+(*
+A refinement based formal specification and information flow security proofs 
+for ARINC 653 compliant separation kernels
+created by Yongwang ZHAO
+School of Computer Science and Engineering, Nanyang Technological University, Singapore
+School of Computer Science and Engineering, Beihang University, China
+zhaoyongwang@gmail.com, ywzhao@ntu.edu.sg, zhaoyw@buaa.edu.cn
+*)
+
+section {* Second-level specification and security proofs *}
+
+theory SK_L2Spec
+imports SK_SecurityModel SK_TopSpec
+
+begin
+
+declare [[ smt_timeout = 90 ]]
+
+subsection {* Definitions *}
+
+subsubsection {* Data type, basic components, and state *}
+
+type_synonym process_id = nat
+datatype process_state =  DORMANT | READY | WAITING | SUSPEND | RUNNING
+
+type_synonym proc_priority_type = nat
+
+record Proc_State = state :: process_state
+                    priority :: proc_priority_type
+
+record StateR = State + 
+                procs :: "partition_id \<rightharpoonup> (process_id set)"
+                cur_proc_part :: "partition_id \<rightharpoonup> process_id"
+                proc_state :: "partition_id \<times> process_id \<rightharpoonup> Proc_State"
+
+definition abstract_state :: "StateR \<Rightarrow> State" ("\<Up>_" [50])        
+  where "abstract_state r = \<lparr>current = current r,
+                            partitions = partitions r,
+                            comm = comm r,
+                            part_ports = part_ports r
+                           \<rparr>"
+
+definition abstract_state_rev :: "StateR \<Rightarrow> State \<Rightarrow> StateR" ("_\<Down>_" [50])
+  where "abstract_state_rev r' r = r'\<lparr>current := current r,
+                            partitions := partitions r,
+                            comm := comm r,
+                            part_ports := part_ports r\<rparr>"
+
+subsubsection {* Events *}
+
+datatype Hypercall' = Create_Sampling_Port port_name
+                     | Write_Sampling_Message port_id Message
+                     | Read_Sampling_Message port_id
+                     | Get_Sampling_Portid port_name
+                     | Get_Sampling_Portstatus port_id
+                     | Create_Queuing_Port port_name
+                     | Send_Queuing_Message port_id Message
+                     | Receive_Queuing_Message port_id
+                     | Get_Queuing_Portid port_name
+                     | Get_Queuing_Portstatus port_id
+                     | Clear_Queuing_Port port_id
+                     | Set_Partition_Mode partition_mode_type
+                     | Get_Partition_Status
+                     | Create_Process proc_priority_type
+                     | Start_Process process_id
+                     | Stop_Process process_id
+                     | Resume_Process process_id
+                     | Suspend_Process process_id
+                     | Set_Priority process_id proc_priority_type
+                     | Get_Process_Status process_id
+
+datatype System_EventR = Schedule
+                        | Transfer_Sampling_Message Channel_Type
+                        | Transfer_Queuing_Message Channel_Type
+                        | Schedule_Process
+
+datatype EventR = hyperc' Hypercall' | sys' System_EventR 
+
+subsubsection{* Event specification *}
+
+definition create_sampling_portR :: "Sys_Config \<Rightarrow> StateR \<Rightarrow> port_name \<Rightarrow> (StateR \<times> port_id option)" where
+  "create_sampling_portR sc s p \<equiv> let s'= (create_sampling_port sc (\<Up>s) p) in (s\<Down>(fst s'),snd s')"
+
+definition write_sampling_messageR :: "StateR \<Rightarrow> port_id \<Rightarrow> Message \<Rightarrow> (StateR \<times> bool)" where
+  "write_sampling_messageR s p m \<equiv> let s'= (write_sampling_message (\<Up>s) p m) in (s\<Down>(fst s'),snd s')"
+
+definition read_sampling_messageR :: "StateR \<Rightarrow> port_id \<Rightarrow> (StateR \<times> Message option)" where
+  "read_sampling_messageR s pid \<equiv> let s'= (read_sampling_message (\<Up>s) pid) in (s\<Down>(fst s'),snd s')"
+
+definition get_sampling_port_idR :: "Sys_Config \<Rightarrow> StateR \<Rightarrow> port_name \<Rightarrow> (StateR \<times> port_id option)" where
+  "get_sampling_port_idR sc s pname \<equiv> let s'= (get_sampling_port_id sc (\<Up>s) pname) in (s\<Down>(fst s'),snd s')"
+
+definition get_sampling_port_statusR :: "Sys_Config \<Rightarrow> StateR \<Rightarrow> port_id \<Rightarrow> (StateR \<times> Port_Type option)" where
+  "get_sampling_port_statusR sc s pid \<equiv> let s'= (get_sampling_port_status sc (\<Up>s) pid) in (s\<Down>(fst s'),snd s')"
+
+definition create_queuing_portR :: "Sys_Config \<Rightarrow> StateR \<Rightarrow> port_name \<Rightarrow> (StateR \<times> port_id option)" where
+  "create_queuing_portR sc s p \<equiv> let s'= (create_queuing_port sc (\<Up>s) p) in (s\<Down>(fst s'),snd s')"
+
+definition send_queuing_message_maylostR :: "Sys_Config \<Rightarrow> StateR \<Rightarrow> port_id \<Rightarrow> Message \<Rightarrow> (StateR \<times> bool)" where
+  "send_queuing_message_maylostR sc s p m \<equiv> 
+        let s'= (send_queuing_message_maylost sc (\<Up>s) p m) in (s\<Down>(fst s'),snd s')"
+
+definition receive_queuing_messageR :: "StateR \<Rightarrow> port_id \<Rightarrow> (StateR \<times> Message option)" where
+  "receive_queuing_messageR s pid \<equiv> let s'= (receive_queuing_message (\<Up>s) pid) in (s\<Down>(fst s'),snd s')"
+
+definition get_queuing_port_idR :: "Sys_Config \<Rightarrow> StateR \<Rightarrow> port_name \<Rightarrow> (StateR \<times> port_id option)" where
+  "get_queuing_port_idR sc s pname \<equiv> let s'= (get_queuing_port_id sc (\<Up>s) pname) in (s\<Down>(fst s'),snd s')"
+
+definition get_queuing_port_statusR :: "Sys_Config \<Rightarrow> StateR \<Rightarrow> port_id \<Rightarrow> (StateR \<times> Port_Type option)" where
+  "get_queuing_port_statusR sc s pid \<equiv> let s'= (get_queuing_port_status sc (\<Up>s) pid) in (s\<Down>(fst s'),snd s')"
+
+definition clear_queuing_portR :: "StateR \<Rightarrow> port_id \<Rightarrow> StateR" where
+  "clear_queuing_portR s pid \<equiv> let s'= (clear_queuing_port (\<Up>s) pid) in (s\<Down>s')"
+
+definition setRun2Ready :: "StateR \<Rightarrow> StateR" where
+  "setRun2Ready s \<equiv> if is_a_partition sysconf (current s) \<and> cur_proc_part s (current s) \<noteq> None then
+                      let prs = proc_state s;
+                          cur = the ((cur_proc_part s) (current s));
+                          stt = the (prs (current s, cur)) in
+                       s\<lparr>cur_proc_part := ((cur_proc_part s)) (current s := None),
+                          proc_state := prs((current s, cur) := Some (stt\<lparr>state:=READY\<rparr>))\<rparr>
+                     else s"
+
+definition schedule_process :: "StateR \<Rightarrow> StateR set" where
+  "schedule_process s \<equiv> if is_a_partition sysconf (current s) 
+                            \<and> part_mode (the ((partitions s) (current s))) = NORMAL then
+                          (let s' = setRun2Ready s;
+                              readyprs = {p. p\<in>the (procs s' (current s')) \<and> 
+                                 state (the (proc_state s' (current s',p))) = READY};
+                              selp = SOME p. p\<in>{x. state (the (proc_state s' (current s',x))) = READY \<and>
+                                                   (\<forall>y\<in>readyprs. priority (the (proc_state s' (current s',x))) \<ge>
+                                                                priority (the (proc_state s' (current s',y))))};
+                              st = the ((proc_state s') (current s', selp));
+                              proc_st = proc_state s';
+                              cur_pr = cur_proc_part s' in
+                                  {s'\<lparr>proc_state := proc_st ((current s', selp) := Some (st\<lparr>state := RUNNING\<rparr>)),
+                                     cur_proc_part := cur_pr(current s' := Some selp)\<rparr>})
+                         else
+                          {s}"
+
+definition scheduleR :: "Sys_Config \<Rightarrow> StateR \<Rightarrow> StateR set" where
+  "scheduleR sc s \<equiv> \<Union>s'\<in>schedule sc (\<Up>s). {s\<Down>s'}" 
+
+definition get_partition_statusR :: 
+    "Sys_Config \<Rightarrow> StateR \<Rightarrow> (StateR \<times> (Partition_Conf option) \<times> (Partition_State_Type option))" where
+      "get_partition_statusR sc s \<equiv> let s'= (get_partition_status sc (\<Up>s)) in (s\<Down>(fst s'),snd s')"
+
+definition remove_partition_resources :: "StateR \<Rightarrow> partition_id \<Rightarrow> StateR" where
+  "remove_partition_resources s part \<equiv> 
+          let proc_state' = (\<lambda>(pt, p). if pt = part then None else (proc_state s) (pt,p));
+              procs' = (procs s)(part := None) in
+                s\<lparr>procs := procs', proc_state:=proc_state'\<rparr>" 
+
+definition set_procs_to_normal :: "StateR \<Rightarrow> partition_id \<Rightarrow> StateR" where
+  "set_procs_to_normal s part \<equiv> if is_a_partition sysconf part then
+                                    let prs = proc_state s;
+                                        proc_state' = (\<lambda>(pt, p). 
+                                              (let pst = prs (pt,p) in
+                                                if pt = part \<and> state (the pst) = WAITING 
+                                                then Some ((the pst)\<lparr>state:=READY\<rparr>)
+                                                else prs (pt,p))) in
+                                     s\<lparr>proc_state := proc_state'\<rparr>
+                                   else s"
+
+definition set_partition_modeR :: "Sys_Config \<Rightarrow> StateR \<Rightarrow> partition_mode_type \<Rightarrow> StateR" where
+  "set_partition_modeR sc s m \<equiv> 
+      (if (partconf sc) (current s) \<noteq> None \<and> (partitions s) (current s) \<noteq> None \<and>
+          \<not> (part_mode (the ((partitions s) (current s))) = COLD_START \<and> m = WARM_START) then
+        let pts = partitions s;
+            pstate = the (pts (current s));
+            s' = (if m = NORMAL then 
+                    set_procs_to_normal s (current s) 
+                  else if part_mode (the ((partitions s) (current s))) = NORMAL then
+                    remove_partition_resources s (current s) 
+                  else s )
+        in s'\<lparr>partitions := pts(current s' := Some (pstate\<lparr>part_mode := m\<rparr>))\<rparr>
+      else
+        s)"
+
+
+definition transf_sampling_msgR :: "StateR \<Rightarrow> Channel_Type \<Rightarrow> StateR" where
+  "transf_sampling_msgR s c \<equiv> 
+          let s'= (transf_sampling_msg (\<Up>s) c) in (s\<Down>s')"
+
+definition transf_queuing_msg_maylostR :: "Sys_Config \<Rightarrow> StateR \<Rightarrow> Channel_Type \<Rightarrow> StateR" where
+  "transf_queuing_msg_maylostR sc s c \<equiv>
+          let s'= (transf_queuing_msg_maylost sc (\<Up>s) c) in (s\<Down>s')"
+
+definition create_process :: "StateR \<Rightarrow> proc_priority_type \<Rightarrow> (StateR \<times> process_id option)" where
+  "create_process s pri \<equiv> if part_mode (the ((partitions s) (current s))) = WARM_START 
+                            \<or> part_mode (the ((partitions s) (current s))) = COLD_START
+                           then 
+                            let pid = (SOME p. p \<notin> the ((procs s) (current s)));
+                                procs' = (procs s) ((current s) := Some ((the ((procs s) (current s))) \<union> {pid}));
+                                proc_state' = (proc_state s) ((current s,pid) := Some \<lparr>state = DORMANT, priority = pri\<rparr>) in
+                            (s\<lparr>procs:=procs', proc_state:=proc_state'\<rparr>, Some pid)
+                           else (s, None)"
+
+definition set_process_priority :: "StateR \<Rightarrow> process_id \<Rightarrow> proc_priority_type \<Rightarrow> StateR" where
+  "set_process_priority s p pri \<equiv> 
+        if (proc_state s) (current s, p) \<noteq> None \<and> (state (the ((proc_state s) (current s, p)))) \<noteq> DORMANT then
+            let st = state (the ((proc_state s) (current s, p)));
+                proc_state' = (proc_state s) ((current s,p) := Some \<lparr>state = st, priority = pri\<rparr>) in
+                s\<lparr>proc_state:=proc_state'\<rparr>
+         else s"
+
+definition start_process :: "StateR \<Rightarrow> process_id \<Rightarrow> StateR" where
+  "start_process s p \<equiv> if p \<in> the ((procs s) (current s)) \<and> (proc_state s) (current s, p) \<noteq> None 
+                        \<and> (state (the ((proc_state s) (current s, p)))) = DORMANT then
+                          let st = (if part_mode (the ((partitions s) (current s))) = NORMAL
+                                    then READY 
+                                    else WAITING);
+                              pst = (the ((proc_state s) (current s, p)));
+                              proc_state' = (proc_state s) ((current s, p) := Some (pst \<lparr>state := st\<rparr>)) in
+                                s\<lparr>proc_state:=proc_state'\<rparr>
+                        else s"
+
+definition stop_process :: "StateR \<Rightarrow> process_id \<Rightarrow> StateR" where 
+  "stop_process s p \<equiv> if p \<in> the ((procs s) (current s)) \<and> (proc_state s) (current s, p) \<noteq> None 
+                        \<and> (state (the ((proc_state s) (current s, p)))) \<noteq> DORMANT then
+                         let pri = priority (the ((proc_state s) (current s, p)));
+                             proc_state' = (proc_state s) ((current s, p) := Some \<lparr>state = DORMANT,priority = pri\<rparr>) in
+                                s\<lparr>proc_state:=proc_state'\<rparr>
+                       else s"
+
+definition suspend_process :: "StateR \<Rightarrow> process_id \<Rightarrow> StateR" where 
+  "suspend_process s p \<equiv> if p \<in> the ((procs s) (current s)) \<and> (proc_state s) (current s, p) \<noteq> None 
+                           \<and> (state (the ((proc_state s) (current s, p)))) \<noteq> DORMANT
+                           \<and> (state (the ((proc_state s) (current s, p)))) \<noteq> SUSPEND then
+                           let pri = priority (the ((proc_state s) (current s, p)));
+                             proc_state' = (proc_state s) ((current s, p) := Some \<lparr>state = SUSPEND,priority = pri\<rparr>) in
+                                s\<lparr>proc_state:=proc_state'\<rparr>
+                          else s"
+
+definition resume_process :: "StateR \<Rightarrow> process_id \<Rightarrow> StateR" where 
+  "resume_process s p \<equiv> if p \<in> the ((procs s) (current s)) \<and> (proc_state s) (current s, p) \<noteq> None 
+                           \<and> (state (the ((proc_state s) (current s, p)))) = SUSPEND then
+                           let pri = priority (the ((proc_state s) (current s, p)));
+                               proc_state' = (proc_state s) ((current s, p) := Some \<lparr>state = READY,priority = pri\<rparr>) in
+                                  s\<lparr>proc_state:=proc_state'\<rparr>
+                          else s"
+
+definition get_process_status :: "StateR \<Rightarrow> process_id \<Rightarrow> (StateR \<times> (Proc_State option))" where
+  "get_process_status s p \<equiv> (s,(proc_state s) (current s, p))"
+
+
+
+definition system_initR :: "Sys_Config \<Rightarrow> StateR"
+  where "system_initR sc \<equiv> let s0 = system_init sc in 
+                              \<lparr>current = current s0,
+                                partitions = partitions s0,
+                                comm = comm s0,
+                                part_ports = part_ports s0,
+                                procs = (\<lambda> x. None),
+                                cur_proc_part = (\<lambda> x. None),
+                                proc_state = (\<lambda> x. None)
+                               \<rparr>"
+declare abstract_state_def[cong del] and abstract_state_rev_def[cong del] and 
+        create_sampling_portR_def [cong del] and write_sampling_messageR_def[cong del] and
+        read_sampling_messageR_def[cong del] and get_sampling_port_idR_def[cong del] and
+        get_sampling_port_statusR_def[cong del] and create_queuing_portR_def[cong del] and
+        send_queuing_message_maylostR_def[cong del] and receive_queuing_messageR_def[cong del] and
+        get_queuing_port_idR_def[cong del] and get_queuing_port_statusR_def[cong del] and
+        clear_queuing_portR_def[cong del] and setRun2Ready_def[cong del] and schedule_process_def[cong del] and
+        scheduleR_def[cong del] and get_partition_statusR_def[cong del] and remove_partition_resources_def[cong del] and
+        set_procs_to_normal_def[cong del] and set_partition_modeR_def[cong] and transf_sampling_msgR_def[cong del] and
+        transf_queuing_msg_maylostR_def[cong del] and create_process_def[cong] and set_process_priority_def[cong del] and
+        start_process_def[cong del] and stop_process_def[cong] and suspend_process_def[cong del] and 
+        resume_process_def[cong del]  and get_process_status_def[cong del] and set_partition_mode_def[cong del]
+
+declare abstract_state_def[cong] and abstract_state_rev_def[cong] and 
+        create_sampling_portR_def [cong] and write_sampling_messageR_def[cong] and
+        read_sampling_messageR_def[cong] and get_sampling_port_idR_def[cong] and
+        get_sampling_port_statusR_def[cong] and create_queuing_portR_def[cong] and
+        send_queuing_message_maylostR_def[cong] and receive_queuing_messageR_def[cong] and
+        get_queuing_port_idR_def[cong] and get_queuing_port_statusR_def[cong] and
+        clear_queuing_portR_def[cong] and setRun2Ready_def[cong] and schedule_process_def[cong] and
+        scheduleR_def[cong] and get_partition_statusR_def[cong] and remove_partition_resources_def[cong] and
+        set_procs_to_normal_def[cong] and set_partition_modeR_def[cong] and transf_sampling_msgR_def[cong] and
+        transf_queuing_msg_maylostR_def[cong] and create_process_def[cong] and set_process_priority_def[cong] and
+        start_process_def[cong] and stop_process_def[cong] and suspend_process_def[cong] and 
+        resume_process_def[cong] and get_process_status_def[cong] and set_partition_mode_def[cong] and schedule_def[cong]
+
+subsection{* Instantiation and Its Proofs of Security Model  *}
+
+consts s0r :: StateR
+
+specification (s0r) 
+  s0r_init: "s0r = system_initR sysconf"
+  by simp
+
+primrec event_enabledR :: "StateR \<Rightarrow> EventR \<Rightarrow> bool"
+    where event_enabledR_hc: "event_enabledR s (hyperc' h) = (is_a_partition sysconf (current s) 
+                                        \<and> part_mode (the (partitions s (current s))) \<noteq> IDLE)" |
+          event_enabledR_sys: "event_enabledR s (sys' h) =  (case h of Schedule \<Rightarrow> True |
+                                                 Transfer_Sampling_Message c \<Rightarrow> (current s = transmitter sysconf) |
+                                                 Transfer_Queuing_Message c \<Rightarrow> (current s = transmitter sysconf) |
+                                                 Schedule_Process \<Rightarrow> (is_a_partition sysconf (current s) 
+                                                              \<and> part_mode (the (partitions s (current s))) = NORMAL))" 
+
+definition exec_eventR :: "EventR \<Rightarrow> (StateR \<times> StateR) set" where
+  "exec_eventR e = {(s,s'). s'\<in> (if event_enabledR s e then (
+      case e of hyperc' (Create_Sampling_Port pname) \<Rightarrow> {fst (create_sampling_portR sysconf s pname)} |
+                hyperc' (Write_Sampling_Message p m) \<Rightarrow> {fst (write_sampling_messageR s p m)} |
+                hyperc' (Read_Sampling_Message p) \<Rightarrow> {fst (read_sampling_messageR s p)} |
+                hyperc' (Get_Sampling_Portid pname) \<Rightarrow> {fst (get_sampling_port_idR sysconf s pname)} |
+                hyperc' (Get_Sampling_Portstatus p) \<Rightarrow> {fst (get_sampling_port_statusR sysconf s p)} |
+                hyperc' (Create_Queuing_Port pname) \<Rightarrow> {fst (create_queuing_portR sysconf s pname)} |
+                hyperc' (Send_Queuing_Message p m) \<Rightarrow> {fst (send_queuing_message_maylostR sysconf s p m)} |
+                hyperc' (Receive_Queuing_Message p) \<Rightarrow> {fst (receive_queuing_messageR s p)} |
+                hyperc' (Get_Queuing_Portid pname) \<Rightarrow> {fst (get_queuing_port_idR sysconf s pname)} |
+                hyperc' (Get_Queuing_Portstatus p) \<Rightarrow> {fst (get_queuing_port_statusR sysconf s p)} |
+                hyperc' (Clear_Queuing_Port p) \<Rightarrow> {clear_queuing_portR s p} |
+                hyperc' (Set_Partition_Mode m) \<Rightarrow> {set_partition_modeR sysconf s m} |
+                hyperc' (Get_Partition_Status) \<Rightarrow> {fst (get_partition_statusR sysconf s)} |
+                hyperc' (Create_Process pri) \<Rightarrow> {fst (create_process s pri)} |
+                hyperc' (Start_Process p) \<Rightarrow> {start_process s p} |
+                hyperc' (Stop_Process p) \<Rightarrow> {stop_process s p} |
+                hyperc' (Resume_Process p) \<Rightarrow> {resume_process s p} |
+                hyperc' (Suspend_Process p) \<Rightarrow> {suspend_process s p} |
+                hyperc' (Set_Priority p pri) \<Rightarrow> {set_process_priority s p pri} |
+                hyperc' (Get_Process_Status p) \<Rightarrow> {fst (get_process_status s p)} |
+                sys' Schedule \<Rightarrow> scheduleR sysconf s |
+                sys' (Transfer_Sampling_Message c) \<Rightarrow> {transf_sampling_msgR s c} |
+                sys' (Transfer_Queuing_Message c) \<Rightarrow> {transf_queuing_msg_maylostR sysconf s c} |
+                sys' (Schedule_Process) \<Rightarrow> schedule_process s )
+                    else {s})}"
+
+definition eR :: "EventR \<Rightarrow> Event option" where
+  "eR e \<equiv> 
+      case e of hyperc' (Create_Sampling_Port pname) \<Rightarrow> Some (hyperc (Hypercall.Create_Sampling_Port pname)) |
+                hyperc' (Write_Sampling_Message p m) \<Rightarrow> Some (hyperc (Hypercall.Write_Sampling_Message p m)) |
+                hyperc' (Read_Sampling_Message p) \<Rightarrow> Some (hyperc (Hypercall.Read_Sampling_Message p)) |
+                hyperc' (Get_Sampling_Portid pname) \<Rightarrow> Some (hyperc (Hypercall.Get_Sampling_Portid pname)) |
+                hyperc' (Get_Sampling_Portstatus p) \<Rightarrow> Some (hyperc (Hypercall.Get_Sampling_Portstatus p)) |
+                hyperc' (Create_Queuing_Port pname) \<Rightarrow> Some (hyperc (Hypercall.Create_Queuing_Port pname)) |
+                hyperc' (Send_Queuing_Message p m) \<Rightarrow> Some (hyperc (Hypercall.Send_Queuing_Message p m)) |
+                hyperc' (Receive_Queuing_Message p) \<Rightarrow> Some (hyperc (Hypercall.Receive_Queuing_Message p)) |
+                hyperc' (Get_Queuing_Portid pname) \<Rightarrow> Some (hyperc (Hypercall.Get_Queuing_Portid pname)) |
+                hyperc' (Get_Queuing_Portstatus p) \<Rightarrow> Some (hyperc (Hypercall.Get_Queuing_Portstatus p)) |
+                hyperc' (Clear_Queuing_Port p) \<Rightarrow> Some (hyperc (Hypercall.Clear_Queuing_Port p)) |
+                hyperc' (Set_Partition_Mode m) \<Rightarrow> Some (hyperc (Hypercall.Set_Partition_Mode m)) |
+                hyperc' (Get_Partition_Status) \<Rightarrow> Some (hyperc (Hypercall.Get_Partition_Status)) |
+                hyperc' (Create_Process pri) \<Rightarrow> None |
+                hyperc' (Start_Process p) \<Rightarrow> None |
+                hyperc' (Stop_Process p) \<Rightarrow> None |
+                hyperc' (Resume_Process p) \<Rightarrow> None |
+                hyperc' (Suspend_Process p) \<Rightarrow> None |
+                hyperc' (Set_Priority p pri) \<Rightarrow> None |
+                hyperc' (Get_Process_Status p) \<Rightarrow> None |
+                sys' Schedule \<Rightarrow>  Some (sys (System_Event.Schedule)) |
+                sys' (Transfer_Sampling_Message c) \<Rightarrow> Some (sys (System_Event.Transfer_Sampling_Message c)) |
+                sys' (Transfer_Queuing_Message c) \<Rightarrow> Some (sys (System_Event.Transfer_Queuing_Message c)) |
+                sys' (Schedule_Process) \<Rightarrow> None "
+
+primrec domain_of_eventR :: "StateR \<Rightarrow> EventR \<Rightarrow> domain_id option"
+  where domain_of_eventR_hc: "domain_of_eventR s (hyperc' h) = Some (current s)" |
+        domain_of_eventR_sys: "domain_of_eventR s (sys' h) =  (case h of Schedule \<Rightarrow> Some (scheduler sysconf) |
+                                                 Transfer_Sampling_Message c \<Rightarrow> Some (transmitter sysconf) |
+                                                 Transfer_Queuing_Message c \<Rightarrow> Some (transmitter sysconf) |
+                                                 Schedule_Process \<Rightarrow> Some (current s) )" 
+
+lemma domain_domainR : "eR e \<noteq> None \<Longrightarrow> domain_of_eventR s e = domain_of_event (\<Up>s) (the (eR e))"
+  proof(induct e)
+    case (hyperc' x) then show ?case
+      proof(induct x) qed(simp add:eR_def)+          
+  next
+    case (sys' x) then show ?case 
+      proof(induct x) qed(simp add:eR_def)+
+  qed
+    
+definition vpeq_part_procs :: "StateR \<Rightarrow> domain_id \<Rightarrow> StateR \<Rightarrow> bool" ("(_ \<sim>. _ .\<sim>\<^sub>\<Delta> _)")
+  where "vpeq_part_procs s d t \<equiv> if is_a_partition sysconf d then 
+                                      ((procs s) d = (procs t) d) \<and>
+                                      (\<forall>p. (proc_state s) (d,p) = (proc_state t) (d,p)) \<and>
+                                      (cur_proc_part s) d = (cur_proc_part t) d 
+                                  else True" 
+
+lemma vpeq_part_procs_transitive_lemma : 
+  "\<forall> s t r d. (vpeq_part_procs s d t) \<and> (vpeq_part_procs t d r) \<longrightarrow> (vpeq_part_procs s d r)"
+  using vpeq_part_procs_def by auto
+  
+lemma vpeq_part_procs_symmetric_lemma : "\<forall> s t d. (vpeq_part_procs s d t) \<longrightarrow> (vpeq_part_procs t d s)"
+  using vpeq_part_procs_def by auto
+
+lemma vpeq_part_procs_reflexive_lemma : "\<forall> s d. (vpeq_part_procs s d s)"
+  using vpeq_part_procs_def by auto
+
+definition vpeqR :: "StateR \<Rightarrow> domain_id \<Rightarrow> StateR \<Rightarrow> bool" ("(_ \<sim>. _ .\<sim> _)")
+  where "vpeqR s d t \<equiv>  ((\<Up>s) \<sim>d\<sim> (\<Up>t)) \<and> (s\<sim>.d.\<sim>\<^sub>\<Delta>t)"
+
+declare vpeqR_def[cong] and vpeq_part_procs_def[cong]
+
+lemma vpeqR_transitive_lemma : "\<forall> s t r d. (vpeqR s d t) \<and> (vpeqR t d r) \<longrightarrow> (vpeqR s d r)"
+    apply(clarsimp cong del: vpeq1_def)
+    using vpeq1_transitive_lemma vpeq_part_procs_transitive_lemma by blast
+
+lemma vpeqR_symmetric_lemma : "\<forall> s t d. (vpeqR s d t) \<longrightarrow> (vpeqR t d s)"
+  apply(clarsimp cong del: vpeq1_def)
+  using vpeq1_symmetric_lemma vpeq_part_procs_symmetric_lemma by blast
+
+lemma vpeqR_reflexive_lemma : "\<forall> s d. (vpeqR s d s)"  
+  using vpeq1_reflexive_lemma vpeq_part_procs_reflexive_lemma by auto
+
+lemma vpeqR_vpeq1 : "vpeqR s d t \<Longrightarrow> vpeq1 (\<Up>s) d (\<Up>t)"
+  by fastforce
+
+lemma sched_currentR_lemma : 
+  "\<forall>s t a. vpeqR s (scheduler sysconf) t \<longrightarrow> (domain_of_eventR s a) = (domain_of_eventR t a)"  
+    using vpeqR_def vpeq1_def abstract_state_def vpeq_sched_def 
+    by (metis (no_types, lifting) EventR.exhaust State.select_convs(1) domain_of_eventR.simps) 
+
+lemma scheproc_hasnexts: "schedule_process s \<noteq> {}"
+  apply(case_tac "is_a_partition sysconf (current s) \<and> part_mode (the ((partitions s) (current s))) = NORMAL")    
+  by auto
+  
+lemma reachable_l2: "\<forall>s a. (SM.reachable0 s0r exec_eventR) s \<longrightarrow> (\<exists>s'. (s, s') \<in> exec_eventR a)"
+  proof -
+  {
+    fix s a
+    assume p0: "(SM.reachable0 s0r exec_eventR) s"
+    have "\<exists>s'. (s, s') \<in> exec_eventR a"
+      proof(induct a)
+        case (hyperc' x) show ?case 
+          proof(induct x) qed(auto simp add:exec_eventR_def)
+        next
+        case (sys' x) then show ?case
+          proof(induct x) 
+            case (Schedule) show ?case using exec_eventR_def  by fastforce
+            case (Transfer_Sampling_Message c) show ?case  using exec_eventR_def  by fastforce
+            case (Transfer_Queuing_Message c) show ?case  using exec_eventR_def  by fastforce
+            case (Schedule_Process) show ?case using exec_eventR_def scheproc_hasnexts by fastforce
+          qed
+      qed        
+  }
+  then show ?thesis by auto
+  qed
+
+
+interpretation SM_enabled 
+    s0r exec_eventR domain_of_eventR "scheduler sysconf" vpeqR interference1
+  using vpeqR_transitive_lemma vpeqR_symmetric_lemma vpeqR_reflexive_lemma sched_currentR_lemma
+        schedeler_intf_all_help no_intf_sched_help reachable_l2 nintf_reflx
+        SM.intro[of vpeqR "scheduler sysconf" domain_of_eventR interference1]
+        SM_enabled_axioms.intro [of s0r exec_eventR]
+        SM_enabled.intro[of domain_of_eventR "scheduler sysconf" vpeqR interference1 s0r exec_eventR] by blast
+
+subsection{* Unwinding conditions on new state variables *}
+  definition weak_step_consistent_new :: "bool" where
+    "weak_step_consistent_new \<equiv> \<forall>a d s t. reachable0 s \<and> reachable0 t \<and> (s \<sim>. d .\<sim> t) \<and> (s \<sim>. (scheduler sysconf) .\<sim> t) \<and> 
+                            ((the (domain_of_eventR s a)) \<leadsto> d) \<and> (s \<sim>. (the (domain_of_eventR s a)) .\<sim> t) \<longrightarrow>
+                            (\<forall> s' t'. (s,s') \<in> exec_eventR a \<and> (t,t') \<in> exec_eventR a \<longrightarrow> (s' \<sim>.d.\<sim>\<^sub>\<Delta> t'))"
+
+  definition step_consistent_new :: "bool" where
+    "step_consistent_new \<equiv> \<forall>a d s t. reachable0 s \<and> reachable0 t \<and> (s \<sim>. d .\<sim> t) \<and> (s \<sim>. (scheduler sysconf) .\<sim> t) \<and> 
+                            ((the (domain_of_eventR s a)) \<leadsto> d) \<longrightarrow> (s \<sim>. (the (domain_of_eventR s a)) .\<sim> t) \<longrightarrow>
+                            (\<forall> s' t'. (s,s') \<in> exec_eventR a \<and> (t,t') \<in> exec_eventR a \<longrightarrow> (s' \<sim>.d.\<sim>\<^sub>\<Delta> t'))"
+
+  definition local_respect_new :: "bool" where
+    "local_respect_new \<equiv> \<forall> a d s s'. reachable0 s \<and> ((the (domain_of_eventR s a)) \<setminus>\<leadsto> d) \<and> (s,s')\<in>exec_eventR a 
+                                    \<longrightarrow> (s \<sim>. d .\<sim>\<^sub>\<Delta> s')"
+
+  definition weak_step_consistent_new_e :: "EventR \<Rightarrow> bool" where
+    "weak_step_consistent_new_e a \<equiv> \<forall>d s t. reachable0 s \<and> reachable0 t \<and> (s \<sim>. d .\<sim> t) \<and> (s \<sim>. (scheduler sysconf) .\<sim> t) \<and> 
+                            ((the (domain_of_eventR s a)) \<leadsto> d) \<and> (s \<sim>. (the (domain_of_eventR s a)) .\<sim> t) \<longrightarrow>
+                            (\<forall> s' t'. (s,s') \<in> exec_eventR a \<and> (t,t') \<in> exec_eventR a \<longrightarrow> (s' \<sim>.d.\<sim>\<^sub>\<Delta> t'))"
+
+  definition step_consistent_new_e :: "EventR \<Rightarrow> bool" where
+    "step_consistent_new_e a \<equiv> \<forall>d s t. reachable0 s \<and> reachable0 t \<and> (s \<sim>. d .\<sim> t) \<and> (s \<sim>. (scheduler sysconf) .\<sim> t) \<and> 
+                            ((the (domain_of_eventR s a)) \<leadsto> d) \<longrightarrow> (s \<sim>. (the (domain_of_eventR s a)) .\<sim> t) \<longrightarrow>
+                            (\<forall> s' t'. (s,s') \<in> exec_eventR a \<and> (t,t') \<in> exec_eventR a \<longrightarrow> (s' \<sim>.d.\<sim>\<^sub>\<Delta> t'))"
+
+  definition local_respect_new_e :: "EventR \<Rightarrow> bool" where
+    "local_respect_new_e a \<equiv> \<forall>d s s'. reachable0 s \<and> ((the (domain_of_eventR s a)) \<setminus>\<leadsto> d) \<and> (s,s')\<in>exec_eventR a 
+                                    \<longrightarrow> (s \<sim>. d .\<sim>\<^sub>\<Delta> s')"
+
+declare weak_step_consistent_new_def[cong del] and step_consistent_new_def[cong del] and local_respect_new_def[cong del] and
+        weak_step_consistent_new_e_def[cong del] and step_consistent_new_e_def[cong del] and local_respect_new_e_def[cong del] 
+
+declare weak_step_consistent_new_def[cong] and step_consistent_new_def[cong] and local_respect_new_def[cong] and
+        weak_step_consistent_new_e_def[cong] and step_consistent_new_e_def[cong] and local_respect_new_e_def[cong] 
+
+declare weak_step_consistent_new_def[cong del] and step_consistent_new_def[cong del] and local_respect_new_def[cong del] and
+        weak_step_consistent_new_e_def[cong del] and step_consistent_new_e_def[cong del] and local_respect_new_e_def[cong del]
+
+  lemma weak_step_consistent_new_all_evt : "weak_step_consistent_new = (\<forall>a. weak_step_consistent_new_e a)"
+    by (simp add:weak_step_consistent_new_def weak_step_consistent_new_e_def)
+
+  lemma step_consistent_new_all_evt : "step_consistent_new = (\<forall>a. step_consistent_new_e a)"
+    by (simp add:step_consistent_new_def step_consistent_new_e_def)
+
+  lemma local_respect_new_all_evt : "local_respect_new = (\<forall>a. local_respect_new_e a)"
+    by (simp add:local_respect_new_def local_respect_new_e_def)
+
+subsection{* Proofs of refinement *}
+
+subsubsection{* Refinement of existing events at upper level *}
+
+  lemma create_sampling_port_ref_lemma: 
+    "\<forall>s. fst (create_sampling_port sc (\<Up>s) p) = \<Up>(fst (create_sampling_portR sc s p))"
+    by auto
+
+  lemma write_sampling_message_ref_lemma: 
+    "\<forall>s. fst (write_sampling_message (\<Up>s) p m) = \<Up>(fst (write_sampling_messageR s p m))"
+    by simp
+  
+  lemma read_sampling_message_ref_lemma: 
+    "\<forall>s. fst (read_sampling_message (\<Up>s) p) = \<Up>(fst (read_sampling_messageR s p))"
+    by simp
+
+  lemma get_sampling_port_id_ref_lemma: 
+    "\<forall>s. fst (get_sampling_port_id sc (\<Up>s) p) = \<Up>(fst (get_sampling_port_idR sc s p))"
+    by simp
+
+  lemma get_sampling_port_status_ref_lemma: 
+    "\<forall>s. fst (get_sampling_port_status sc (\<Up>s) p) = \<Up>(fst (get_sampling_port_statusR sc s p))"
+    by simp
+  
+  lemma create_queuing_port_ref_lemma: 
+    "\<forall>s. fst (create_queuing_port sc (\<Up>s) p) = \<Up>(fst (create_queuing_portR sc s p))"
+    by auto 
+
+  lemma send_queuing_message_maylost_ref_lemma: 
+    "\<forall>s. fst (send_queuing_message_maylost sc (\<Up>s) p m) = \<Up>(fst (send_queuing_message_maylostR sc s p m))"
+    by simp 
+
+  lemma receive_queuing_message_ref_lemma: 
+    "\<forall>s. fst (receive_queuing_message (\<Up>s) p) = \<Up>(fst (receive_queuing_messageR s p))"
+      by auto
+
+  lemma get_queuing_port_id_ref_lemma: 
+    "\<forall>s. fst (get_queuing_port_id sc (\<Up>s) p) = \<Up>(fst (get_queuing_port_idR sc s p))"
+      by auto
+
+  lemma get_queuing_port_status_ref_lemma: 
+    "\<forall>s. fst (get_queuing_port_status sc (\<Up>s) p) = \<Up>(fst (get_queuing_port_statusR sc s p))"
+      by auto
+
+  lemma clear_queuing_port_ref_lemma: 
+    "\<forall>s. clear_queuing_port (\<Up>s) p = \<Up>(clear_queuing_portR s p)"
+      by auto
+
+  lemma schedule_ref_lemma: "\<forall>s s'. (s' \<in> scheduleR sc s) \<longrightarrow> (\<Up>s') \<in> (schedule sc (\<Up>s))"
+     by auto
+
+  lemma get_partition_status_ref_lemma: 
+    "\<forall>s. fst (get_partition_status sc (\<Up>s)) = \<Up>(fst (get_partition_statusR sc s))"
+     by simp
+
+  lemma set_partition_mode_ref_lemma: "\<forall>s. set_partition_mode sc (\<Up>s) m = \<Up>(set_partition_modeR sc s m)"
+    proof -
+    {
+      fix s
+      let ?s' = "set_partition_modeR sc s m"
+      let ?us' = "\<Up>(?s')"
+      let ?t = "\<Up>s"
+      let ?t' = "set_partition_mode sc ?t m"
+      have a0: "current ?t' = current ?us'" 
+        using set_partition_mode_def 
+          by auto
+      moreover
+      have "partitions ?t' = partitions ?us'"
+        proof -
+          have b0: "partitions s = partitions ?t \<and> current s = current ?t"
+            by simp
+          {
+            fix p
+            have "partitions ?t' p = partitions ?us' p"
+              proof(cases "(partconf sc) (current s) \<noteq> None \<and> (partitions s) (current s) \<noteq> None \<and>
+                    \<not> (part_mode (the ((partitions s) (current s))) = COLD_START \<and> m = WARM_START)")
+                assume c0: "(partconf sc) (current s) \<noteq> None \<and> (partitions s) (current s) \<noteq> None \<and>
+                    \<not> (part_mode (the ((partitions s) (current s))) = COLD_START \<and> m = WARM_START)"
+                with b0 have c1: "(partconf sc) (current ?t) \<noteq> None \<and> (partitions ?t) (current ?t) \<noteq> None \<and>
+                    \<not> (part_mode (the ((partitions ?t) (current ?t))) = COLD_START \<and> m = WARM_START)"
+                  by simp
+                show ?thesis 
+                  proof(cases "current ?t = p")
+                    assume d0: "current ?t = p"                      
+                    with c1 have "partitions ?t' p = Some ((the (partitions ?t p)) \<lparr>part_mode := m\<rparr>)" 
+                      by auto 
+                    moreover
+                    from b0 c0 d0 have "partitions ?s' p = Some ((the (partitions s p)) \<lparr>part_mode := m\<rparr>)"
+                      by auto
+                    ultimately show ?thesis by (auto cong del: set_partition_mode_def)
+                  next
+                    assume d0: "current ?t \<noteq> p"                    
+                    with c1 have "partitions ?t' p = partitions ?t p" 
+                      by auto 
+                    moreover
+                    from b0 c0 d0 have "partitions ?s' p = partitions s p"
+                       by auto 
+                    ultimately show ?thesis by auto
+                  qed
+              next
+                assume c0: "\<not> ((partconf sc) (current s) \<noteq> None \<and> (partitions s) (current s) \<noteq> None \<and>
+                    \<not> (part_mode (the ((partitions s) (current s))) = COLD_START \<and> m = WARM_START))"
+                thus ?thesis  by auto
+              qed                  
+          }
+          then show ?thesis by auto
+      qed
+      thus ?thesis  by auto
+    } qed
+
+
+
+  lemma transf_sampling_msg_ref_lemma: "\<forall>s. transf_sampling_msg (\<Up>s) c = \<Up>(transf_sampling_msgR s c)"
+    by auto
+
+  lemma transf_queuing_msg_maylost_ref_lemma: 
+    "\<forall>s. transf_queuing_msg_maylost sc (\<Up>s) c = \<Up>(transf_queuing_msg_maylostR sc s c)"
+      by auto
+
+subsubsection{* new events introduced at this level dont change abstract state *}
+  lemma setrun2ready_nchastate_lemma: 
+    "s' = setRun2Ready s \<Longrightarrow> (\<Up>s) = (\<Up>s')" 
+    by auto
+
+  lemma schedule_process_nchastate_lemma: 
+    "\<forall>s'\<in>(schedule_process s). (\<Up>s) = (\<Up>s')" 
+     proof -
+     {
+       fix s'
+       assume p0: "s'\<in>(schedule_process s)"
+       
+       let ?s' = "setRun2Ready s"
+        let ?readyprs = "{p. p\<in>the (procs ?s' (current ?s')) \<and> 
+                                state (the (proc_state ?s' (current ?s',p))) = READY}"
+        have "(\<Up>s) = (\<Up>s')"
+          proof(cases "is_a_partition sysconf (current s)  \<and> part_mode (the ((partitions s) (current s))) = NORMAL")
+            assume a0: "is_a_partition sysconf (current s)  \<and> part_mode (the ((partitions s) (current s))) = NORMAL"
+            let ?s' = "setRun2Ready s"
+            have b2: "(\<Up>s) = (\<Up>?s')" using setrun2ready_nchastate_lemma by blast
+            have b3: "(\<Up>?s') = (\<Up>s')" using  a0 p0 by auto               
+            with b2 show ?thesis by (auto cong del: abstract_state_def setRun2Ready_def)
+        next
+          assume a0: "\<not> (is_a_partition sysconf (current s)  \<and> part_mode (the ((partitions s) (current s))) = NORMAL)"
+          then show ?thesis using p0 by auto
+        qed
+    }
+    then show ?thesis  by (auto cong del: abstract_state_def )
+    qed
+
+
+  lemma create_process_nchastate_lemma: 
+    "\<forall>s. (\<Up>s) = \<Up>(fst (create_process s pri))" 
+     by auto
+
+  lemma set_process_priority_nchastate_lemma: 
+    "\<forall>s. (\<Up>s) = \<Up>(set_process_priority s p pri)" 
+      by auto
+
+  lemma start_process_nchastate_lemma: 
+    "\<forall>s. (\<Up>s) = \<Up>(start_process s p)" 
+      by auto
+
+  lemma stop_process_nchastate_lemma: 
+    "\<forall>s. (\<Up>s) = \<Up>(stop_process s p)" 
+      by auto
+
+  lemma suspend_process_nchastate_lemma: 
+    "\<forall>s. (\<Up>s) = \<Up>(suspend_process s p)" 
+      by auto
+  
+  lemma resume_process_nchastate_lemma: 
+    "\<forall>s. (\<Up>s) = \<Up>(resume_process s p)" 
+     by auto
+
+  lemma get_process_status_nchastate_lemma: 
+    "\<forall>s. (\<Up>s) = \<Up>(fst (get_process_status s p))" 
+     by auto
+
+subsubsection{* proof of refinement *}
+  
+  lemma s0_ref_lemma : "(\<Up>s0r) = s0t" 
+     by (simp add:  s0t_init s0r_init system_initR_def ) 
+
+  lemma refine_exec_event : "(s,t)\<in>exec_eventR e \<Longrightarrow> (eR e = None \<longrightarrow> (\<Up>s) = (\<Up>t)) 
+    \<and> (eR e \<noteq> None \<longrightarrow> (\<Up>s,\<Up>t)\<in>exec_event (the (eR e)))"
+    proof -
+      assume p0: "(s,t)\<in>exec_eventR e"
+      then show "(eR e = None \<longrightarrow> (\<Up>s) = (\<Up>t)) \<and> (eR e \<noteq> None \<longrightarrow> (\<Up>s,\<Up>t)\<in>exec_event (the (eR e)))"
+      proof(induct e)
+        case (hyperc' x) then show ?case
+          proof(induct x)
+            case (Create_Sampling_Port y) 
+              let ?e = "Hypercall.Create_Sampling_Port y"
+              let ?er = "Create_Sampling_Port y"
+              have "event_enabledR s (hyperc' ?er) = event_enabled (\<Up>s) (hyperc ?e)"
+                 by auto
+              then have "((\<Up>s),(\<Up>t)) \<in> exec_event (hyperc ?e)" 
+                  using create_sampling_port_ref_lemma exec_eventR_def exec_event_def 
+                  Create_Sampling_Port.prems  
+                  by (auto cong del: abstract_state_def)
+              then show ?case using eR_def by auto
+          next
+            case (Write_Sampling_Message x1 y)
+              let ?e = "Hypercall.Write_Sampling_Message x1 y"
+              let ?er = "Write_Sampling_Message x1 y"
+              have "event_enabledR s (hyperc' ?er) = event_enabled (\<Up>s) (hyperc ?e)"
+                using event_enabled_def abstract_state_def by auto
+              then have "((\<Up>s),(\<Up>t)) \<in> exec_event (hyperc ?e)" 
+                  using write_sampling_message_ref_lemma exec_eventR_def exec_event_def 
+                     Write_Sampling_Message.prems
+                   by (auto cong del: abstract_state_def) 
+              then show ?case using eR_def by auto
+          next
+            case (Read_Sampling_Message y)
+              let ?e = "Hypercall.Read_Sampling_Message y"
+              let ?er = "Read_Sampling_Message y"
+              have "event_enabledR s (hyperc' ?er) = event_enabled (\<Up>s) (hyperc ?e)"
+                using event_enabled_def abstract_state_def by auto
+              then have "((\<Up>s),(\<Up>t)) \<in> exec_event (hyperc ?e)" 
+                  using read_sampling_message_ref_lemma exec_eventR_def exec_event_def 
+                     Read_Sampling_Message.prems by (auto cong del: abstract_state_def)
+              then show ?case using eR_def by auto
+          next
+            case (Get_Sampling_Portid y)
+              let ?e = "Hypercall.Get_Sampling_Portid y"
+              let ?er = "Get_Sampling_Portid y"
+              have "event_enabledR s (hyperc' ?er) = event_enabled (\<Up>s) (hyperc ?e)"
+                using event_enabled_def abstract_state_def by auto
+              then have "((\<Up>s),(\<Up>t)) \<in> exec_event (hyperc ?e)" 
+                  using get_sampling_port_id_ref_lemma exec_eventR_def exec_event_def 
+                     Get_Sampling_Portid by (auto cong del: abstract_state_def) 
+              then show ?case using eR_def by auto
+          next
+            case (Get_Sampling_Portstatus y)
+              let ?e = "Hypercall.Get_Sampling_Portstatus y"
+              let ?er = "Get_Sampling_Portstatus y"
+              have "event_enabledR s (hyperc' ?er) = event_enabled (\<Up>s) (hyperc ?e)"
+                using event_enabled_def abstract_state_def by auto
+              then have "((\<Up>s),(\<Up>t)) \<in> exec_event (hyperc ?e)" 
+                  using get_sampling_port_status_ref_lemma exec_eventR_def exec_event_def 
+                     Get_Sampling_Portstatus.prems by (auto cong del: abstract_state_def)
+              then show ?case using eR_def by auto
+          next
+            case (Create_Queuing_Port y)
+              let ?e = "Hypercall.Create_Queuing_Port y"
+              let ?er = "Create_Queuing_Port y"
+              have "event_enabledR s (hyperc' ?er) = event_enabled (\<Up>s) (hyperc ?e)"
+                using event_enabled_def abstract_state_def by auto
+              then have "((\<Up>s),(\<Up>t)) \<in> exec_event (hyperc ?e)" 
+                  using create_queuing_port_ref_lemma exec_eventR_def exec_event_def 
+                     Create_Queuing_Port.prems by (auto cong del: abstract_state_def)
+              then show ?case using eR_def by auto
+          next
+            case (Send_Queuing_Message x1 y1)
+              let ?e = "Hypercall.Send_Queuing_Message x1 y1"
+              let ?er = "Send_Queuing_Message x1 y1"
+              have "event_enabledR s (hyperc' ?er) = event_enabled (\<Up>s) (hyperc ?e)"
+                using event_enabled_def abstract_state_def by auto
+              then have "((\<Up>s),(\<Up>t)) \<in> exec_event (hyperc ?e)" 
+                  using send_queuing_message_maylost_ref_lemma exec_eventR_def exec_event_def 
+                     Send_Queuing_Message.prems by (auto cong del: abstract_state_def)
+              then show ?case using eR_def by auto
+          next
+             case (Receive_Queuing_Message x1)
+              let ?e = "Hypercall.Receive_Queuing_Message x1"
+              let ?er = "Receive_Queuing_Message x1"
+              have "event_enabledR s (hyperc' ?er) = event_enabled (\<Up>s) (hyperc ?e)"
+                using event_enabled_def abstract_state_def by auto
+              then have "((\<Up>s),(\<Up>t)) \<in> exec_event (hyperc ?e)" 
+                  using receive_queuing_message_ref_lemma exec_eventR_def exec_event_def 
+                     Receive_Queuing_Message.prems by (auto cong del: abstract_state_def)
+              then show ?case using eR_def by auto
+          next
+            case (Get_Queuing_Portid x1)
+              let ?e = "Hypercall.Get_Queuing_Portid x1"
+              let ?er = "Get_Queuing_Portid x1"
+              have "event_enabledR s (hyperc' ?er) = event_enabled (\<Up>s) (hyperc ?e)"
+                using event_enabled_def abstract_state_def by auto
+              then have "((\<Up>s),(\<Up>t)) \<in> exec_event (hyperc ?e)" 
+                  using get_queuing_port_id_ref_lemma exec_eventR_def exec_event_def 
+                     Get_Queuing_Portid.prems by (auto cong del: abstract_state_def) 
+              then show ?case using eR_def by auto
+          next
+            case (Get_Queuing_Portstatus x1)
+              let ?e = "Hypercall.Get_Queuing_Portstatus x1"
+              let ?er = "Get_Queuing_Portstatus x1"
+              have "event_enabledR s (hyperc' ?er) = event_enabled (\<Up>s) (hyperc ?e)"
+                using event_enabled_def abstract_state_def by auto
+              then have "((\<Up>s),(\<Up>t)) \<in> exec_event (hyperc ?e)" 
+                  using get_queuing_port_status_ref_lemma exec_eventR_def exec_event_def 
+                     Get_Queuing_Portstatus.prems by (auto cong del: abstract_state_def) 
+              then show ?case using eR_def by auto
+          next
+            case (Clear_Queuing_Port x1)
+              let ?e = "Hypercall.Clear_Queuing_Port x1"
+              let ?er = "Clear_Queuing_Port x1"
+              have "event_enabledR s (hyperc' ?er) = event_enabled (\<Up>s) (hyperc ?e)"
+                using event_enabled_def abstract_state_def by auto
+              then have "((\<Up>s),(\<Up>t)) \<in> exec_event (hyperc ?e)" 
+                  using clear_queuing_port_ref_lemma exec_eventR_def exec_event_def 
+                     Clear_Queuing_Port.prems by (auto cong del: abstract_state_def)
+              then show ?case using eR_def by auto
+          next
+            case (Set_Partition_Mode x1)
+              let ?e = "Hypercall.Set_Partition_Mode x1"
+              let ?er = "Set_Partition_Mode x1"
+              have "event_enabledR s (hyperc' ?er) = event_enabled (\<Up>s) (hyperc ?e)"
+                using event_enabled_def abstract_state_def by auto
+              then have "((\<Up>s),(\<Up>t)) \<in> exec_event (hyperc ?e)" 
+                  using set_partition_mode_ref_lemma exec_eventR_def exec_event_def 
+                     Set_Partition_Mode.prems 
+                     by (auto cong del: set_partition_modeR_def 
+                              abstract_state_def event_enabledR_def 
+                               event_enabled_def set_partition_mode_def)
+              then show ?case using eR_def by auto
+          next
+            case (Get_Partition_Status)
+              let ?e = "Hypercall.Get_Partition_Status"
+              let ?er = "Get_Partition_Status"
+              have "event_enabledR s (hyperc' ?er) = event_enabled (\<Up>s) (hyperc ?e)"
+                using event_enabled_def abstract_state_def by auto
+              then have "((\<Up>s),(\<Up>t)) \<in> exec_event (hyperc ?e)" 
+                  using get_partition_status_ref_lemma exec_eventR_def exec_event_def 
+                     Get_Partition_Status.prems by (auto cong del: abstract_state_def) 
+              then show ?case using eR_def by auto
+          next
+            case (Create_Process x1) 
+              let ?er = "Create_Process x1"
+              show ?case using eR_def exec_eventR_def Create_Process.prems create_process_nchastate_lemma                  
+                by (metis (no_types, lifting) EventR.simps(5) Hypercall'.simps(413) 
+                    mem_Collect_eq old.prod.case singletonD)
+          next
+            case (Start_Process x1)
+              let ?er = "Start_Process x1"
+              show ?case using eR_def exec_eventR_def Start_Process.prems start_process_nchastate_lemma
+                by (metis (no_types, lifting) EventR.simps(5) Hypercall'.simps(414) 
+                    mem_Collect_eq old.prod.case singletonD)
+          next
+            case (Stop_Process x1)
+              let ?er = "Stop_Process x1"
+              show ?case using eR_def exec_eventR_def Stop_Process.prems stop_process_nchastate_lemma
+                by (metis (no_types, lifting) EventR.simps(5) Hypercall'.simps(415) 
+                    mem_Collect_eq old.prod.case singletonD)
+          next
+            case (Resume_Process x1)
+              let ?er = "Resume_Process x1"
+              show ?case using eR_def exec_eventR_def Resume_Process.prems resume_process_nchastate_lemma
+                by (metis (no_types, lifting) EventR.simps(5) Hypercall'.simps(416) 
+                    mem_Collect_eq old.prod.case singletonD)
+          next
+            case (Suspend_Process x1)
+              let ?er = "Suspend_Process x1"
+              show ?case using eR_def exec_eventR_def Suspend_Process.prems suspend_process_nchastate_lemma
+                by (metis (no_types, lifting) EventR.simps(5) Hypercall'.simps(417) 
+                    mem_Collect_eq old.prod.case singletonD)
+          next
+            case (Set_Priority x1 y1)
+              let ?er = "Set_Priority x1 y1"
+              show ?case using eR_def exec_eventR_def Set_Priority.prems set_process_priority_nchastate_lemma
+                by (metis (no_types, lifting) EventR.simps(5) Hypercall'.simps(418) 
+                    mem_Collect_eq old.prod.case singletonD)
+          next
+            case (Get_Process_Status x1)
+              let ?er = "Get_Process_Status x1"
+              show ?case using eR_def exec_eventR_def Get_Process_Status.prems get_process_status_nchastate_lemma
+                by (metis (no_types, lifting) EventR.simps(5) Hypercall'.simps(419) 
+                    mem_Collect_eq old.prod.case singletonD)
+          qed
+      next
+        case (sys' x) then show ?case 
+          proof(induct x)
+            case (Schedule)
+              let ?e = "System_Event.Schedule"
+              let ?er = "Schedule"
+              have "event_enabledR s (sys' ?er) = event_enabled (\<Up>s) (sys ?e)"
+                by auto
+              then have "((\<Up>s),(\<Up>t)) \<in> exec_event (sys ?e)" 
+                  using schedule_ref_lemma exec_eventR_def exec_event_def 
+                     Schedule.prems by (auto cong del:  scheduleR_def) 
+              then show ?case using eR_def by auto
+          next
+            case (Transfer_Sampling_Message x1)
+              let ?e = "System_Event.Transfer_Sampling_Message x1"
+              let ?er = "Transfer_Sampling_Message x1"
+              have "event_enabledR s (sys' ?er) = event_enabled (\<Up>s) (sys ?e)"
+                 by auto
+              then have "((\<Up>s),(\<Up>t)) \<in> exec_event (sys ?e)" 
+                  using transf_sampling_msg_ref_lemma exec_eventR_def exec_event_def 
+                     Transfer_Sampling_Message.prems by auto 
+              then show ?case using eR_def by auto
+          next
+            case (Transfer_Queuing_Message x1)
+              let ?e = "System_Event.Transfer_Queuing_Message x1"
+              let ?er = "Transfer_Queuing_Message x1"
+              have "event_enabledR s (sys' ?er) = event_enabled (\<Up>s) (sys ?e)"
+                 by auto
+              then have "((\<Up>s),(\<Up>t)) \<in> exec_event (sys ?e)" 
+                  using transf_queuing_msg_maylost_ref_lemma exec_eventR_def exec_event_def 
+                     Transfer_Queuing_Message.prems  by auto 
+              then show ?case using eR_def by auto
+          next
+            case (Schedule_Process)
+              let ?er = "Schedule_Process"
+              show ?case using eR_def exec_eventR_def Schedule_Process.prems schedule_process_nchastate_lemma
+                by (metis (no_types, lifting) EventR.simps(6) System_EventR.simps(18) 
+                   prod.simps(2) mem_Collect_eq singletonD) 
+        qed
+      qed
+  qed
+
+  lemma reachR_reach1: 
+     "\<forall>s as s'. SK_TopSpec.reachable0 (\<Up>s) \<and> 
+                 reachable0 s \<and> s'\<in>execute as s  \<longrightarrow> 
+                SK_TopSpec.reachable0 (\<Up>s')"
+  proof -
+  {
+    fix as
+    have "\<forall>s s'. SK_TopSpec.reachable0 (\<Up>s) \<and> reachable0 s \<and> s'\<in>execute as s
+                        \<longrightarrow> SK_TopSpec.reachable0 (\<Up>s')"
+    proof(induct as)
+      case Nil show ?case using execute_def by fastforce
+    next
+      case (Cons b bs)
+      assume a0: "\<forall>s s'. SK_TopSpec.reachable0 (\<Up>s) \<and> reachable0 s \<and> s'\<in>execute bs s
+                      \<longrightarrow> SK_TopSpec.reachable0 (\<Up>s')"
+      show ?case 
+      proof -
+      {
+        fix s s'
+        assume b0: "SK_TopSpec.reachable0 (\<Up>s) \<and> reachable0 s \<and> s'\<in>execute (b # bs) s"
+        have b2: "current s = current (\<Up>s) \<and> partitions s = partitions (\<Up>s)" by (simp add:abstract_state_def)
+        have b3: "\<forall>s1. (s,s1)\<in>exec_eventR b \<longrightarrow> SK_TopSpec.reachable0 (\<Up>s1)"
+        proof -
+        {
+          fix s1
+          assume c0: "(s,s1)\<in>exec_eventR b"
+          then have "SK_TopSpec.reachable0 (\<Up>s1)"
+            using SK_TopSpec.reachableStep b0 refine_exec_event by metis 
+        }
+        then show ?thesis by auto
+        qed
+        from b0 have "\<exists>s1. (s,s1)\<in>exec_eventR b \<and> (s1,s')\<in>run bs" using execute_def 
+          by (simp add: relcomp.simps)
+        then obtain s1 where b4: "(s,s1)\<in>exec_eventR b \<and> (s1,s')\<in>run bs" by auto
+        with b3 have b5: "SK_TopSpec.reachable0 (\<Up>s1)" by simp
+        have b6: "SK_L2Spec.reachable0 s1" using SK_L2Spec.reachableStep b0 b4 by blast 
+        with b4 b5 a0 have "SK_TopSpec.reachable0 (\<Up>s')" using execute_def by auto
+      } then show ?thesis by auto
+      qed
+    qed
+  } then show ?thesis by auto
+  qed
+
+
+lemma reachR_reach: "reachable0 s \<Longrightarrow> SK_TopSpec.reachable0 (\<Up>s)" 
+  using reachR_reach1 SK_L2Spec.reachable0_def reachable_s0 SK_TopSpec.reachable_s0 s0_ref_lemma
+    by (metis Image_singleton_iff execute_def reachable_def)
+
+primrec rmtau :: "'a option list => 'a list"
+  where "rmtau [] = []" |
+        "rmtau (a#as) = (if a \<noteq> None then
+                          the a # rmtau as
+                         else rmtau as)"
+
+lemma refine_sound_helper: "\<forall>es st sr. st = \<Up>sr \<longrightarrow> 
+          (image abstract_state (execute es sr)) \<subseteq> (SK_TopSpec.execute (rmtau (map eR es)) st)"
+  proof -
+  {
+    fix es
+    have "\<forall>st sr. st = \<Up>sr \<longrightarrow> 
+          (image abstract_state (execute es sr)) \<subseteq> (SK_TopSpec.execute (rmtau (map eR es)) st)"
+    proof(induct es)
+      case Nil show ?case
+      proof -
+      {
+        fix st sr
+        assume a0: "st = \<Up>sr"
+        then have "abstract_state ` SK_L2Spec.execute [] sr = {st}" 
+          using SK_L2Spec.execute_def by auto            
+        moreover
+        from a0 have "SK_TopSpec.execute (rmtau (map eR [])) st = {st}" 
+          using SK_TopSpec.execute_def SK_L2Spec.run.run_Nil by simp
+        ultimately have "abstract_state ` SK_L2Spec.execute [] sr \<subseteq> SK_TopSpec.execute (rmtau (map eR [])) st" 
+          by blast
+      } then show ?thesis by auto qed
+      next
+        case (Cons a as)
+        assume a0: "\<forall>st sr. st = \<Up>sr \<longrightarrow> 
+              abstract_state ` SK_L2Spec.execute as sr \<subseteq> SK_TopSpec.execute (rmtau (map eR as)) st"
+        show ?case
+        proof -
+        {
+          fix st sr
+          assume b0: "st = \<Up>sr"
+          have b1: "SK_L2Spec.execute (a # as) sr = Image (exec_eventR a O run as) {sr}" 
+            using SK_L2Spec.execute_def SK_L2Spec.run.run_Cons by simp
+          
+          have "abstract_state ` SK_L2Spec.execute (a # as) sr \<subseteq> SK_TopSpec.execute (rmtau (map eR (a # as))) st"
+          proof(cases "eR a = None")
+            assume c0: "eR a = None"
+            then have c1:"rmtau (map eR (a # as)) = rmtau (map eR as)" 
+              using rmtau_def by simp
+            let ?nextsr = "SK_L2Spec.next_states sr a"
+            have c2:"Image (exec_eventR a O run as) {sr} = Image (run as) ?nextsr" 
+              using SK_L2Spec.next_states_def by auto
+            {
+              fix s
+              assume d0: "s\<in>abstract_state ` SK_L2Spec.execute (a # as) sr"
+              with b1 c2 have "\<exists>s'\<in>?nextsr. s\<in>abstract_state ` Image (run as) {s'}"
+                by auto  
+              then obtain s' where d1:"s'\<in>?nextsr \<and> s\<in>abstract_state ` Image (run as) {s'}" by auto
+              from c0 d1 have d2: "st = \<Up>s'" using refine_exec_event SK_L2Spec.next_states_def 
+                b0 by auto 
+              with a0 have "abstract_state ` SK_L2Spec.execute as s' \<subseteq> SK_TopSpec.execute (rmtau (map eR as)) st"
+                by simp
+              with c1 d1 have "s\<in>SK_TopSpec.execute (rmtau (map eR (a # as))) st" 
+                using SK_L2Spec.execute_def subsetCE by auto 
+            }
+            then show ?thesis by blast
+          next
+            assume c0: "eR a \<noteq> None"
+            then have c1:"rmtau (map eR (a # as)) = (the (eR a)) # (rmtau (map eR as))" 
+              using rmtau_def by simp
+            let ?nextsr = "SK_L2Spec.next_states sr a"
+            let ?nextst = "SK_TopSpec.next_states st (the (eR a))"
+            have c2:"Image (exec_eventR a O run as) {sr} = Image (run as) ?nextsr" 
+              using SK_L2Spec.next_states_def by auto
+            have c3:"Image (exec_event (the (eR a)) O SK_TopSpec.run (rmtau (map eR as))) {st} 
+                  = Image (SK_TopSpec.run (rmtau (map eR as))) ?nextst" 
+              using SK_TopSpec.next_states_def by auto
+            {
+              fix s
+              assume d0: "s\<in>abstract_state ` SK_L2Spec.execute (a # as) sr"
+              with b1 c2 have "\<exists>s'\<in>?nextsr. s\<in>abstract_state ` Image (run as) {s'}"
+                using Image_singleton_iff SK_L2Spec.next_states_def imageE 
+                  image_eqI mem_Collect_eq relcomp.cases by auto
+              then obtain s' where d1:"s'\<in>?nextsr \<and> s\<in>abstract_state ` Image (run as) {s'}" by auto
+              from c0 d1 have "\<exists>st'\<in>?nextst. st' = \<Up>s'" using refine_exec_event SK_L2Spec.next_states_def 
+                b0 by (simp add: SK_TopSpec.next_states_def) 
+              then obtain st' where d2: "st'\<in>?nextst \<and> st' = \<Up>s'" by auto
+              from a0 d1 d2 have "abstract_state ` SK_L2Spec.execute as s' \<subseteq> SK_TopSpec.execute (rmtau (map eR as)) st'"
+                by simp
+              with c1 c2 c3 d1 d2 have "s\<in>SK_TopSpec.execute (rmtau (map eR (a # as))) st" 
+                using SK_L2Spec.execute_def ImageI Image_singleton_iff SK_TopSpec.execute_def 
+                  SK_TopSpec.run.run_Cons subsetCE by auto  
+            }
+            then show ?thesis by fastforce
+          qed
+        }
+        then show ?thesis by blast
+        qed
+      qed
+    }
+    then show ?thesis by auto
+    qed
+
+theorem refine_sound: "(image abstract_state (execute es s0r)) \<subseteq> (SK_TopSpec.execute (rmtau (map eR es)) s0t)"
+  using refine_sound_helper s0_ref_lemma by fastforce 
+
+subsubsection{* unwinding conditions of refinement*}
+
+  lemma weak_step_consistent_new_evt_ref: 
+    "\<forall>e. eR e = None \<and> weak_step_consistent_new_e e \<longrightarrow> SK_L2Spec.weak_step_consistent_e e"
+      by (metis SK_L2Spec.weak_step_consistent_e_def refine_exec_event vpeqR_def 
+          weak_step_consistent_new_e_def)
+    
+  lemma local_respect_new_evt_ref: 
+    "\<forall>e. eR e = None \<and> local_respect_new_e e \<longrightarrow> SK_L2Spec.local_respect_e e"
+      using SK_L2Spec.local_respect_e_def SK_TopSpec.non_interference_def 
+        local_respect_new_e_def non_interference1_def refine_exec_event 
+        vpeqR_def vpeqR_reflexive_lemma by metis
+   
+  lemma weak_step_consistent_evt_ref: 
+    "\<forall>e. eR e \<noteq> None \<and> SK_TopSpec.weak_step_consistent_e (the (eR e)) 
+          \<and> weak_step_consistent_new_e e \<longrightarrow> SK_L2Spec.weak_step_consistent_e e"    
+    by (smt SK_L2Spec.weak_step_consistent_e_def SK_TopSpec.step_consistent_def 
+        SK_TopSpec.weak_with_step_cons domain_domainR local_respect reachR_reach 
+        refine_exec_event vpeqR_def vpeqR_vpeq1 weak_step_consistent weak_step_consistent_new_e_def)
+    
+  lemma local_respect_evt_ref: 
+    "\<forall>e. eR e \<noteq> None \<and> SK_TopSpec.local_respect_e (the (eR e)) 
+          \<and> local_respect_new_e e \<longrightarrow> SK_L2Spec.local_respect_e e"
+    using SK_L2Spec.local_respect_e_def SK_TopSpec.local_respect_e_def 
+          SK_TopSpec.non_interference_def domain_domainR local_respect_new_e_def 
+          non_interference1_def reachR_reach refine_exec_event vpeqR_def by metis
+
+  lemma abs_sc_new_imp: "\<lbrakk>SK_TopSpec.weak_step_consistent; weak_step_consistent_new\<rbrakk> 
+        \<Longrightarrow> SK_L2Spec.weak_step_consistent"
+    using SK_L2Spec.weak_step_consistent_all_evt SK_TopSpec.weak_step_consistent_all_evt 
+            weak_step_consistent_evt_ref weak_step_consistent_new_all_evt 
+              weak_step_consistent_new_evt_ref by blast 
+
+  lemma abs_lr_new_imp: "\<lbrakk>SK_TopSpec.local_respect; local_respect_new\<rbrakk> \<Longrightarrow> SK_L2Spec.local_respect"
+    using SK_L2Spec.local_respect_all_evt SK_TopSpec.local_respect_all_evt 
+      local_respect_evt_ref local_respect_new_all_evt local_respect_new_evt_ref by blast
+    
+  theorem noninfl_refinement: "\<lbrakk>SK_TopSpec.local_respect; SK_TopSpec.weak_step_consistent; 
+              weak_step_consistent_new; local_respect_new\<rbrakk> \<Longrightarrow> noninfluence"
+    using SK_L2Spec.UnwindingTheorem1 SK_L2Spec.noninf_eq_noninf_gen 
+            abs_lr_new_imp abs_sc_new_imp by metis 
+    
+subsection{* Existing events preserve "local respect" on new state variables *} 
+
+subsubsection{*proving "create sampling port"*}
+
+  lemma crt_smpl_portR_presrv_lcrsp_new:
+      assumes p3:"s' = fst (create_sampling_portR sysconf s pname)"
+      shows   "s \<sim>. d .\<sim>\<^sub>\<Delta> s'" using p3 by fastforce    
+
+  lemma crt_smpl_portR_presrv_lcrsp_new_e: "local_respect_new_e (hyperc' (Create_Sampling_Port pn))"
+    using crt_smpl_portR_presrv_lcrsp_new local_respect_new_e_def exec_eventR_def 
+    by fastforce 
+
+subsubsection{*proving "write sampling message"*}
+
+  lemma write_smpl_msgR_presrv_lcrsp_new:
+    assumes p3:"s' = fst (write_sampling_messageR s pid m)"
+    shows   "s \<sim>. d .\<sim>\<^sub>\<Delta> s'"
+    using p3  by fastforce 
+  
+
+  lemma write_smpl_msgR_presrv_lcrsp_new_e: "local_respect_new_e (hyperc' (Write_Sampling_Message p m))"
+    using write_smpl_msgR_presrv_lcrsp_new local_respect_new_e_def exec_eventR_def 
+    by fastforce 
+
+subsubsection{*proving "read sampling message"*}
+
+  lemma read_smpl_msgR_presrv_lcrsp_new:
+      assumes p3:"s' = fst (read_sampling_messageR s pid)"
+      shows   "s \<sim>. d .\<sim>\<^sub>\<Delta> s'"
+    using p3  by fastforce 
+
+  lemma read_smpl_msgR_presrv_lcrsp_new_e: "local_respect_new_e (hyperc' (Read_Sampling_Message p))"
+    using read_smpl_msgR_presrv_lcrsp_new local_respect_new_e_def exec_eventR_def 
+    by fastforce
+
+subsubsection{*proving "get sampling portid"*}
+
+  lemma get_smpl_pidR_presrv_lcrsp_new:
+      assumes p3:"s' = fst (get_sampling_port_idR sysconf s pname)"
+      shows   "s \<sim>. d .\<sim>\<^sub>\<Delta> s'"
+     using p3 by fastforce
+
+  lemma get_smpl_pidR_presrv_lcrsp_new_e: "local_respect_new_e (hyperc' (Get_Sampling_Portid p))"
+    using get_smpl_pidR_presrv_lcrsp_new local_respect_new_e_def exec_eventR_def 
+    by fastforce
+
+subsubsection{*proving "get sampling port status"*}
+  lemma get_smpl_pstsR_presrv_lcrsp_new:
+      assumes p3:"s' = fst (get_sampling_port_statusR sysconf s pid)"
+      shows   "s \<sim>. d .\<sim>\<^sub>\<Delta> s'"
+      using p3 by fastforce
+
+  lemma get_smpl_pstsR_presrv_lcrsp_new_e: "local_respect_new_e (hyperc' (Get_Sampling_Portstatus p))"
+    using get_smpl_pstsR_presrv_lcrsp_new local_respect_new_e_def exec_eventR_def 
+      by fastforce
+
+subsubsection{*proving "create queuing port"*}
+  lemma crt_que_portR_presrv_lcrsp_new:
+  assumes p3:"s' = fst (create_queuing_portR sysconf s pname)"
+  shows   "s \<sim>. d .\<sim>\<^sub>\<Delta> s'"
+  using p3 by fastforce
+   
+  lemma crt_que_portR_presrv_lcrsp_new_e: "local_respect_new_e (hyperc' (Create_Queuing_Port p))"
+    using crt_que_portR_presrv_lcrsp_new local_respect_new_e_def exec_eventR_def 
+    by fastforce
+
+subsubsection{*proving "send queuing message(may lost)"*}
+  lemma snd_que_msg_lstR_presrv_lcrsp_new:
+    assumes p3:"s' = fst (send_queuing_message_maylostR sysconf s pid m)"
+    shows   "s \<sim>. d .\<sim>\<^sub>\<Delta> s'"
+    using p3 by fastforce
+  
+
+  lemma snd_que_msg_lstR_presrv_lcrsp_new_e: "local_respect_new_e (hyperc' (Send_Queuing_Message p m))"
+    using snd_que_msg_lstR_presrv_lcrsp_new local_respect_new_e_def exec_eventR_def 
+     by fastforce
+
+subsubsection{*proving "receive queuing message"*}
+  lemma rec_que_msgR_presrv_lcrsp_new:
+      assumes p3:"s' = fst (receive_queuing_messageR s pid)"
+      shows   "s \<sim>. d .\<sim>\<^sub>\<Delta> s'"
+      using p3 by fastforce
+
+  lemma rec_que_msgR_presrv_lcrsp_new_e: "local_respect_new_e (hyperc' (Receive_Queuing_Message p))"
+    using rec_que_msgR_presrv_lcrsp_new local_respect_new_e_def exec_eventR_def 
+     by fastforce
+
+subsubsection{*proving "get queuing portid"*}
+  lemma get_que_pidR_presrv_lcrsp_new:
+      assumes p3:"s' = fst (get_queuing_port_idR sysconf s pname)"
+      shows   "s \<sim>. d .\<sim>\<^sub>\<Delta> s'"
+      using p3 by fastforce
+
+  lemma get_que_pidR_presrv_lcrsp_new_e: "local_respect_new_e (hyperc' (Get_Queuing_Portid p))"
+    using get_que_pidR_presrv_lcrsp_new local_respect_new_e_def exec_eventR_def 
+    by fastforce
+
+subsubsection{*proving "get queuing port status"*}
+  lemma get_que_pstsR_presrv_lcrsp_new:
+      assumes p3:"s' = fst (get_queuing_port_statusR sysconf s pid)"
+      shows   "s \<sim>. d .\<sim>\<^sub>\<Delta> s'"
+    using p3 by fastforce
+
+  lemma get_que_pstsR_presrv_lcrsp_new_e: "local_respect_new_e (hyperc' (Get_Queuing_Portstatus p))"
+    using get_que_pstsR_presrv_lcrsp_new local_respect_new_e_def exec_eventR_def 
+    by fastforce
+
+subsubsection{*proving "clear queuing port"*}
+  lemma clr_que_portR_presrv_lcrsp_new:
+      assumes p3:"s' = clear_queuing_portR s pid"
+      shows   "s \<sim>. d .\<sim>\<^sub>\<Delta> s'"
+      using p3 by fastforce
+
+  lemma clr_que_portR_presrv_lcrsp_new_e: "local_respect_new_e (hyperc' (Clear_Queuing_Port p))"
+    using clr_que_portR_presrv_lcrsp_new local_respect_new_e_def exec_eventR_def 
+    by fastforce
+
+subsubsection{*proving "get partition statue"*}
+  lemma get_part_statusR_presrv_lcrsp_new:
+      assumes p3:"s' = fst (get_partition_statusR sysconf s)"
+      shows   "s \<sim>. d .\<sim>\<^sub>\<Delta> s'"
+   using p3 by fastforce 
+   
+
+  lemma get_part_statusR_presrv_lcrsp_new_e: "local_respect_new_e (hyperc' Get_Partition_Status)"
+    using get_part_statusR_presrv_lcrsp_new local_respect_new_e_def exec_eventR_def
+      vpeq_part_procs_reflexive_lemma by (fastforce cong del: vpeq_part_procs_def) 
+
+subsubsection{*proving "set partition mode"*}
+  lemma set_procs_to_normal_presrv_lcrsp_new:
+    assumes p3: "current s \<noteq> d"
+      and   p4: "s' = set_procs_to_normal s (current s)"
+      shows   "s \<sim>. d .\<sim>\<^sub>\<Delta> s'"
+      using p3 p4   by auto 
+
+
+  lemma remove_partition_resources_presrv_lcrsp_new:
+    assumes p3: "current s \<noteq> d"
+      and   p4: "s' = remove_partition_resources s (current s)"
+      shows   "s \<sim>. d .\<sim>\<^sub>\<Delta> s'" 
+      using p3 p4  by auto 
+
+  lemma set_part_modeR_presrv_lcrsp_new:
+    assumes 
+         p3: "current s \<noteq> d"
+      and   p4: "s' = set_partition_modeR sysconf s m"
+      shows   "s \<sim>. d .\<sim>\<^sub>\<Delta> s'"
+    using p3 p4 by auto
+
+  lemma set_part_modeR_presrv_lcrsp_new_e: "local_respect_new_e (hyperc' (Set_Partition_Mode p))"
+    using set_part_modeR_presrv_lcrsp_new local_respect_new_e_def 
+      exec_eventR_def nintf_neq domain_of_eventR_hc event_enabledR_hc   
+   by (fastforce cong del: set_partition_modeR_def non_interference1_def )
+    
+subsubsection{*proving "schedule" *}
+  lemma scheduleR_presrv_lcrsp_new:
+      assumes p2:"(scheduler sysconf) \<setminus>\<leadsto> d"       
+      shows   "s \<sim>. d .\<sim>\<^sub>\<Delta> s'"
+    using p2 schedeler_intf_all_help by auto
+
+  lemma scheduleR_presrv_lcrsp_new_e: "local_respect_new_e (sys' Schedule)"
+    using scheduleR_presrv_lcrsp_new local_respect_new_e_def 
+      exec_eventR_def nintf_neq domain_of_eventR_hc event_enabledR_hc  
+    by (auto cong del: non_interference1_def)
+
+subsubsection{*proving "Transfer Sampling Message"*}
+  lemma trans_smpl_msgR_presrv_lcrsp_new:
+      assumes p3:"s' = transf_sampling_msgR s c"
+      shows   "s \<sim>. d .\<sim>\<^sub>\<Delta> s'"
+   using p3 by fastforce
+
+  lemma trans_smpl_msgR_presrv_lcrsp_new_e: "local_respect_new_e (sys' (Transfer_Sampling_Message c))"
+    using trans_smpl_msgR_presrv_lcrsp_new local_respect_new_e_def 
+      exec_eventR_def nintf_neq 
+      domain_of_eventR_hc event_enabledR_hc  
+   by (fastforce cong del: non_interference1_def)
+
+subsubsection{*proving "Transfer Queuing Message"*}
+  lemma trans_que_msg_mlostR_presrv_lcrsp_new:
+      assumes p3:"s' = transf_queuing_msg_maylostR sysconf s c"
+      shows   "s \<sim>. d .\<sim>\<^sub>\<Delta> s'" 
+    using p3 by fastforce
+
+  lemma trans_que_msg_mlostR_presrv_lcrsp_new_e: "local_respect_new_e (sys' (Transfer_Queuing_Message c))"
+    using trans_que_msg_mlostR_presrv_lcrsp_new local_respect_new_e_def 
+      exec_eventR_def nintf_neq domain_of_eventR_hc event_enabledR_hc 
+    by (fastforce cong del: non_interference1_def) 
+
+subsection{* New events preserve "local respect" on new state variables *} 
+lemma create_process_vpeq_part_procs:
+    assumes 
+           p3: "current s \<noteq> d"
+      and  p4: "s' = fst (create_process s pri)"
+    shows "s \<sim>. d .\<sim>\<^sub>\<Delta> s'" 
+    using  p3 p4  by auto   
+
+lemma create_process_presrv_lcrsp_new_e: "local_respect_new_e (hyperc' (Create_Process p))"
+  using create_process_vpeq_part_procs local_respect_new_e_def 
+    exec_eventR_def nintf_neq 
+    domain_of_eventR_hc event_enabledR_hc  
+   by (auto cong del: create_process_def non_interference1_def) 
+
+lemma set_process_priority_vpeq_part_procs:
+    assumes 
+           p3: "current s \<noteq> d"
+      and  p4: "s' = set_process_priority s p pri"
+    shows "s \<sim>. d .\<sim>\<^sub>\<Delta> s'" 
+   using  p3 p4 by auto
+
+lemma set_process_priority_presrv_lcrsp_new_e: "local_respect_new_e (hyperc' (Set_Priority p pri))"
+  using set_process_priority_vpeq_part_procs local_respect_new_e_def 
+    exec_eventR_def nintf_neq vpeq_part_procs_def
+  by (auto cong del:  non_interference1_def set_process_priority_def)
+
+lemma start_process_vpeq_part_procs:
+    assumes p3: "current s \<noteq> d"
+      and  p4: "s' = start_process s p"
+    shows "s \<sim>. d .\<sim>\<^sub>\<Delta> s'" 
+    using  p3 p4 by auto
+
+lemma start_process_presrv_lcrsp_new_e: "local_respect_new_e (hyperc' (Start_Process p))"
+  using start_process_vpeq_part_procs local_respect_new_e_def 
+    exec_eventR_def nintf_neq  
+   by (auto cong del: non_interference1_def start_process_def)
+
+lemma stop_process_vpeq_part_procs:
+    assumes 
+           p3: "current s \<noteq> d"
+      and  p4: "s' = stop_process s p"
+    shows "s \<sim>. d .\<sim>\<^sub>\<Delta> s'" 
+    using p3 p4 by auto
+
+lemma stop_process_presrv_lcrsp_new_e: "local_respect_new_e (hyperc' (Stop_Process p))"
+  using stop_process_vpeq_part_procs local_respect_new_e_def 
+    exec_eventR_def nintf_neq  
+   by (auto cong del: stop_process_def non_interference1_def)
+
+lemma suspend_process_vpeq_part_procs:
+    assumes 
+           p3: "current s \<noteq> d"
+      and  p4: "s' = suspend_process s p"
+    shows "s \<sim>. d .\<sim>\<^sub>\<Delta> s'" 
+    using  p3 p4 by auto
+    
+lemma suspend_process_presrv_lcrsp_new_e: "local_respect_new_e (hyperc' (Suspend_Process p))"
+  using suspend_process_vpeq_part_procs local_respect_new_e_def 
+    exec_eventR_def nintf_neq  
+   by (auto cong del: suspend_process_def non_interference1_def)
+
+lemma resume_process_vpeq_part_procs:
+    assumes p3: "current s \<noteq> d"
+      and  p4: "s' = resume_process s p"
+    shows "s \<sim>. d .\<sim>\<^sub>\<Delta> s'" 
+    using p3 p4 by auto
+
+
+lemma resume_process_presrv_lcrsp_new_e: "local_respect_new_e (hyperc' (Resume_Process p))"
+  using resume_process_vpeq_part_procs local_respect_new_e_def 
+    exec_eventR_def nintf_neq vpeq_part_procs_def 
+   by (auto cong del: resume_process_def non_interference1_def)
+
+lemma get_process_status_vpeq_part_procs:
+    assumes 
+            p3: "current s \<noteq> d"
+      and  p4: "s' = fst (get_process_status s p)"
+    shows "s \<sim>. d .\<sim>\<^sub>\<Delta> s'" 
+  using p3 p4 by auto
+
+
+lemma get_process_status_presrv_lcrsp_new_e: "local_respect_new_e (hyperc' (Get_Process_Status p))"
+  using get_process_status_vpeq_part_procs local_respect_new_e_def 
+    exec_eventR_def nintf_neq  
+ by (auto cong del: get_process_status_def non_interference1_def)
+
+
+lemma schedule_process_vpeq_part_procs:
+     assumes p3: "current s \<noteq> d"
+      and  p4: "s' \<in> schedule_process s"
+    shows "s \<sim>. d .\<sim>\<^sub>\<Delta> s'" 
+    proof -
+      let ?s' = "setRun2Ready s"
+      let ?readyprs = "{p. p\<in>the (procs ?s' (current ?s')) \<and> 
+                              state (the (proc_state ?s' (current ?s',p))) = READY}"
+      show ?thesis 
+        proof(cases "is_a_partition sysconf (current s) \<and> part_mode (the ((partitions s) (current s))) = NORMAL")
+          assume a0: "is_a_partition sysconf (current s) \<and> part_mode (the ((partitions s) (current s))) = NORMAL"
+          let ?s' = "setRun2Ready s"
+          let ?readyprs = "{p. p\<in>the (procs ?s' (current ?s')) \<and> 
+                                  state (the (proc_state ?s' (current ?s',p))) = READY}"
+          let ?selp = "SOME p. p\<in>{x. state (the (proc_state ?s' (current ?s',x))) = READY \<and>
+                                                         (\<forall>y\<in>?readyprs. priority (the (proc_state ?s' (current ?s',x))) \<ge>
+                                                                      priority (the (proc_state ?s' (current ?s',y))))}"
+          let ?st = "the ((proc_state ?s') (current ?s', ?selp))"
+          let ?proc_st = "proc_state ?s'"
+          let ?cur_pr = "cur_proc_part ?s'"
+          from a0 have a1: "schedule_process s = {?s'\<lparr>proc_state := ?proc_st ((current ?s', ?selp) := Some (?st\<lparr>state := RUNNING\<rparr>)),
+                                           cur_proc_part := ?cur_pr(current ?s' := Some ?selp)\<rparr>}"
+            by auto
+          then have b2: "vpeq_part_procs s d ?s'" using p3   by auto
+          have b4: "current s = current ?s'"  by auto
+          then have b3: "vpeq_part_procs ?s' d s'"
+            using p3 a1 p4 by(auto cong del: schedule_process_def setRun2Ready_def)                                    
+          with b2 show ?thesis using  vpeq_part_procs_transitive_lemma by blast 
+      next
+        assume a0: "\<not> (is_a_partition sysconf (current s) \<and> part_mode (the ((partitions s) (current s))) = NORMAL)"
+        then show ?thesis using  p4  by auto
+      qed
+  qed
+
+lemma schedule_process_presrv_lcrsp_new_e: "local_respect_new_e (sys' Schedule_Process)"
+  using schedule_process_vpeq_part_procs local_respect_new_e_def 
+    exec_eventR_def nintf_neq domain_of_eventR_hc   
+   by (auto cong del: non_interference1_def schedule_process_def)
+
+subsection{* Proving the "local respect" property on new variables *}
+  theorem local_respect_new:local_respect_new
+  proof -
+      {
+        fix e
+        have "local_respect_new_e e"
+          apply(induct e)
+          using crt_smpl_portR_presrv_lcrsp_new_e write_smpl_msgR_presrv_lcrsp_new_e 
+                  read_smpl_msgR_presrv_lcrsp_new_e get_smpl_pidR_presrv_lcrsp_new_e
+                  get_smpl_pstsR_presrv_lcrsp_new_e crt_que_portR_presrv_lcrsp_new_e
+                  snd_que_msg_lstR_presrv_lcrsp_new_e rec_que_msgR_presrv_lcrsp_new_e
+                  get_que_pidR_presrv_lcrsp_new_e get_que_pstsR_presrv_lcrsp_new_e
+                  clr_que_portR_presrv_lcrsp_new_e set_part_modeR_presrv_lcrsp_new_e
+                  get_part_statusR_presrv_lcrsp_new_e create_process_presrv_lcrsp_new_e     
+                  start_process_presrv_lcrsp_new_e stop_process_presrv_lcrsp_new_e 
+                  resume_process_presrv_lcrsp_new_e suspend_process_presrv_lcrsp_new_e
+                  set_process_priority_presrv_lcrsp_new_e get_process_status_presrv_lcrsp_new_e
+          apply(rule Hypercall'.induct)
+          using scheduleR_presrv_lcrsp_new_e trans_smpl_msgR_presrv_lcrsp_new_e
+                  trans_que_msg_mlostR_presrv_lcrsp_new_e schedule_process_presrv_lcrsp_new_e 
+          by(rule System_EventR.induct)
+      }
+      then show ?thesis using local_respect_new_all_evt by simp
+    qed
+
+subsection{* Existing events preserve "step consistent" on new state variables *} 
+
+  lemma crt_smpl_portR_presrv_wk_stp_cons_new:
+      assumes 
+              p1:"s \<sim>. d .\<sim> t"
+        and   p2:"s' = fst (create_sampling_portR sysconf s pname)"
+        and   p3:"t' = fst (create_sampling_portR sysconf t pname)"
+      shows   "s' \<sim>. d .\<sim>\<^sub>\<Delta> t'" 
+    using p1 p2 p3 by fastforce
+
+  lemma crt_smpl_portR_presrv_wk_stp_cons_new_e: "weak_step_consistent_new_e (hyperc' (Create_Sampling_Port pn))"
+    using crt_smpl_portR_presrv_wk_stp_cons_new weak_step_consistent_new_e_def 
+      exec_eventR_def domain_of_eventR_def event_enabledR_def same_part_mode sched_vpeq
+        non_interference1_def non_interference_def singletonD 
+          by (smt EventR.case(1) Hypercall'.case(1) State.select_convs(1) State.select_convs(2) 
+                abstract_state_def domain_of_eventR_hc event_enabledR_hc mem_Collect_eq 
+                singletonD vpeqR_def option.sel prod.simps(2))
+
+  lemma wrt_smpl_msgR_presrv_wk_stp_cons_new:
+      assumes p1:"s \<sim>. d .\<sim> t"
+        and   p2:"s' = fst (write_sampling_messageR s pid m)"
+        and   p3:"t' = fst (write_sampling_messageR t pid m)"
+      shows   "s' \<sim>. d .\<sim>\<^sub>\<Delta> t'"
+   using p1 p2 p3 by fastforce
+
+  lemma wrt_smpl_msgR_presrv_wk_stp_cons_new_e: "weak_step_consistent_new_e (hyperc' (Write_Sampling_Message p m))"
+    using wrt_smpl_msgR_presrv_wk_stp_cons_new weak_step_consistent_new_e_def 
+      exec_eventR_def domain_of_eventR_def event_enabledR_def same_part_mode sched_vpeq 
+      non_interference1_def non_interference_def singletonD event_enabledR_hc domain_of_eventR_hc
+      abstract_state_def vpeqR_def
+          by (smt EventR.case(1) Hypercall'.case(2) State.select_convs(1) State.select_convs(2) 
+                abstract_state_def mem_Collect_eq singletonD  option.sel prod.simps(2))
+
+  lemma read_smpl_msgR_presrv_wk_stp_cons_new:
+      assumes p1:"s \<sim>. d .\<sim> t"
+        and   p2:"s' = fst (read_sampling_messageR s pid)"
+        and   p3:"t' = fst (read_sampling_messageR t pid)"
+      shows   "s' \<sim>. d .\<sim>\<^sub>\<Delta> t'"  
+   using p1 p2 p3 by fastforce
+
+  lemma read_smpl_msgR_presrv_wk_stp_cons_new_e: "weak_step_consistent_new_e (hyperc' (Read_Sampling_Message p))"
+    using read_smpl_msgR_presrv_wk_stp_cons_new weak_step_consistent_new_e_def 
+      exec_eventR_def domain_of_eventR_def event_enabledR_def same_part_mode sched_vpeq 
+      non_interference1_def non_interference_def singletonD 
+          by (smt EventR.case(1) Hypercall'.case(3) State.select_convs(1) State.select_convs(2) 
+                abstract_state_def domain_of_eventR_hc event_enabledR_hc mem_Collect_eq 
+                singletonD vpeqR_def option.sel prod.simps(2))
+
+  lemma get_smpl_pidR_presrv_wk_stp_cons_new:
+      assumes p1:"s \<sim>. d .\<sim> t"
+        and   p2:"s' = fst (get_sampling_port_idR sysconf s pname)"
+        and   p3:"t' = fst (get_sampling_port_idR sysconf t pname)"
+      shows   "s' \<sim>. d .\<sim>\<^sub>\<Delta> t'" 
+    using p1 p2 p3 by fastforce
+
+
+  lemma get_smpl_pidR_presrv_wk_stp_cons_new_e: "weak_step_consistent_new_e (hyperc' (Get_Sampling_Portid p))"
+    using get_smpl_pidR_presrv_wk_stp_cons_new weak_step_consistent_new_e_def 
+      exec_eventR_def domain_of_eventR_def event_enabledR_def same_part_mode sched_vpeq 
+      non_interference1_def non_interference_def singletonD 
+          by (smt EventR.case(1) Hypercall'.case(4) State.select_convs(1) State.select_convs(2) 
+                abstract_state_def domain_of_eventR_hc event_enabledR_hc mem_Collect_eq 
+                singletonD vpeqR_def option.sel prod.simps(2))
+
+  lemma get_smpl_pstsR_presrv_wk_stp_cons_new:
+      assumes p1:"s \<sim>. d .\<sim> t"
+        and   p2:"s' = fst (get_sampling_port_statusR sysconf s pid)"
+        and   p3:"t' = fst (get_sampling_port_statusR sysconf t pid)"
+      shows   "s' \<sim>. d .\<sim>\<^sub>\<Delta> t'" 
+     using p1 p2 p3 by fastforce
+
+  lemma get_smpl_pstsR_presrv_wk_stp_cons_new_e: "weak_step_consistent_new_e (hyperc' (Get_Sampling_Portstatus p))"
+    using get_smpl_pstsR_presrv_wk_stp_cons_new weak_step_consistent_new_e_def 
+      exec_eventR_def domain_of_eventR_def event_enabledR_def same_part_mode sched_vpeq 
+      non_interference1_def non_interference_def singletonD 
+          by (smt EventR.case(1) Hypercall'.case(5) State.select_convs(1) State.select_convs(2) 
+                abstract_state_def domain_of_eventR_hc event_enabledR_hc mem_Collect_eq 
+                singletonD vpeqR_def option.sel prod.simps(2))
+
+  lemma crt_que_portR_presrv_wk_stp_cons_new:
+      assumes p1:"s \<sim>. d .\<sim> t"
+        and   p2:"s' = fst (create_queuing_portR sysconf s pname)"
+        and   p3:"t' = fst (create_queuing_portR sysconf t pname)"
+      shows   "s' \<sim>. d .\<sim>\<^sub>\<Delta> t'"
+     using p1 p2 p3 by auto
+
+  lemma crt_que_portR_presrv_wk_stp_cons_new_e: "weak_step_consistent_new_e (hyperc' (Create_Queuing_Port p))"
+    using crt_que_portR_presrv_wk_stp_cons_new weak_step_consistent_new_e_def 
+      exec_eventR_def domain_of_eventR_def event_enabledR_def same_part_mode sched_vpeq 
+      non_interference1_def non_interference_def singletonD 
+          by (smt EventR.case(1) Hypercall'.case(6) State.select_convs(1) State.select_convs(2) 
+                abstract_state_def domain_of_eventR_hc event_enabledR_hc mem_Collect_eq 
+                singletonD vpeqR_def option.sel prod.simps(2))
+
+  lemma snd_que_msg_lstR_presrv_wk_stp_cons_new:
+      assumes 
+              p1:"s \<sim>. d .\<sim> t"
+        and   p2:"s' = fst (send_queuing_message_maylostR sysconf s pid m)"
+        and   p3:"t' = fst (send_queuing_message_maylostR sysconf t pid m)"
+      shows   "s' \<sim>. d .\<sim>\<^sub>\<Delta> t'"
+     using p1 p2 p3 by auto
+
+  lemma snd_que_msg_lstR_presrv_wk_stp_cons_new_e: "weak_step_consistent_new_e (hyperc' (Send_Queuing_Message p m))"
+    using snd_que_msg_lstR_presrv_wk_stp_cons_new weak_step_consistent_new_e_def 
+      exec_eventR_def domain_of_eventR_def event_enabledR_def same_part_mode sched_vpeq 
+      non_interference1_def non_interference_def singletonD 
+          by (smt EventR.case(1) Hypercall'.case(7) State.select_convs(1) State.select_convs(2) 
+                abstract_state_def domain_of_eventR_hc event_enabledR_hc mem_Collect_eq 
+                singletonD vpeqR_def option.sel prod.simps(2))
+
+  lemma rec_que_msgR_presrv_wk_stp_cons_new:
+      assumes p1:"s \<sim>. d .\<sim> t"                
+        and   p2:"s' = fst (receive_queuing_messageR s pid)"
+        and   p3:"t' = fst (receive_queuing_messageR t pid)"
+      shows   "s' \<sim>. d .\<sim>\<^sub>\<Delta> t'"
+    using p1 p2 p3 by auto
+
+  lemma rec_que_msgR_presrv_wk_stp_cons_new_e: "weak_step_consistent_new_e (hyperc' (Receive_Queuing_Message p))"
+    using rec_que_msgR_presrv_wk_stp_cons_new weak_step_consistent_new_e_def 
+      exec_eventR_def domain_of_eventR_def event_enabledR_def same_part_mode sched_vpeq 
+      non_interference1_def non_interference_def singletonD 
+          by (smt EventR.case(1) Hypercall'.case(8) State.select_convs(1) State.select_convs(2) 
+                abstract_state_def domain_of_eventR_hc event_enabledR_hc mem_Collect_eq 
+                singletonD vpeqR_def option.sel prod.simps(2))
+
+  lemma get_que_pidR_presrv_wk_stp_cons_new:
+      assumes p1:"s \<sim>. d .\<sim> t"
+        and   p2:"s' = fst (get_queuing_port_idR sysconf s pname)"
+        and   p3:"t' = fst (get_queuing_port_idR sysconf t pname)"
+      shows   "s' \<sim>. d .\<sim>\<^sub>\<Delta> t'" using p1 p2 p3 by auto
+
+  lemma get_que_pidR_presrv_wk_stp_cons_new_e: "weak_step_consistent_new_e (hyperc' (Get_Queuing_Portid p))"
+    using get_que_pidR_presrv_wk_stp_cons_new weak_step_consistent_new_e_def 
+      exec_eventR_def domain_of_eventR_def event_enabledR_def same_part_mode sched_vpeq 
+          by (smt EventR.case(1) Hypercall'.case(9) State.select_convs(1) State.select_convs(2) 
+                abstract_state_def domain_of_eventR_hc event_enabledR_hc mem_Collect_eq 
+                singletonD vpeqR_def option.sel prod.simps(2))
+
+  lemma get_que_pstsR_presrv_wk_stp_cons_new:
+      assumes p1:"s \<sim>. d .\<sim> t"
+        and   p2:"s' = fst (get_queuing_port_statusR sysconf s pid)"
+        and   p3:"t' = fst (get_queuing_port_statusR sysconf t pid)"
+      shows   "s' \<sim>. d .\<sim>\<^sub>\<Delta> t'" using p1 p2 p3 by auto
+
+  lemma get_que_pstsR_presrv_wk_stp_cons_new_e: "weak_step_consistent_new_e (hyperc' (Get_Queuing_Portstatus p))"
+    using get_que_pstsR_presrv_wk_stp_cons_new weak_step_consistent_new_e_def 
+      exec_eventR_def domain_of_eventR_def event_enabledR_def same_part_mode sched_vpeq 
+      non_interference1_def non_interference_def singletonD 
+          by (smt EventR.case(1) Hypercall'.case(10) State.select_convs(1) State.select_convs(2) 
+                abstract_state_def domain_of_eventR_hc event_enabledR_hc mem_Collect_eq 
+                singletonD vpeqR_def option.sel prod.simps(2))
+
+  lemma clr_que_portR_presrv_wk_stp_cons_new:
+      assumes p1:"s \<sim>. d .\<sim> t"
+        and   p2:"s' = clear_queuing_portR s pid"
+        and   p3:"t' = clear_queuing_portR t pid"
+      shows   "s' \<sim>. d .\<sim>\<^sub>\<Delta> t'"
+      using p1 p2 p3 by auto
+
+  lemma clr_que_portR_presrv_wk_stp_cons_new_e: "weak_step_consistent_new_e (hyperc' (Clear_Queuing_Port p))"
+    using clr_que_portR_presrv_wk_stp_cons_new weak_step_consistent_new_e_def 
+      exec_eventR_def domain_of_eventR_def event_enabledR_def same_part_mode sched_vpeq 
+          by (smt EventR.case(1) Hypercall'.case(11) State.select_convs(1) State.select_convs(2) 
+                abstract_state_def domain_of_eventR_hc event_enabledR_hc mem_Collect_eq 
+                singletonD vpeqR_def option.sel prod.simps(2))
+
+  lemma get_part_statusR_presrv_wk_stp_cons_new:
+      assumes p1:"s \<sim>. d .\<sim> t"
+        and   p2:"s' = fst (get_partition_statusR sysconf s)"
+        and   p3:"t' = fst (get_partition_statusR sysconf t)"
+      shows   "s' \<sim>. d .\<sim>\<^sub>\<Delta> t'" using p1 p2 p3 by auto
+
+  lemma get_part_statusR_presrv_wk_stp_cons_new_e: "weak_step_consistent_new_e (hyperc' Get_Partition_Status)"
+    using get_part_statusR_presrv_wk_stp_cons_new weak_step_consistent_new_e_def 
+      exec_eventR_def domain_of_eventR_def event_enabledR_def same_part_mode sched_vpeq 
+          by (smt EventR.case(1) Hypercall'.case(13) State.select_convs(1) State.select_convs(2) 
+                abstract_state_def domain_of_eventR_hc event_enabledR_hc mem_Collect_eq 
+                singletonD vpeqR_def option.sel prod.simps(2))
+
+  lemma scheduleR_presrv_wk_stp_cons_new:
+      assumes p1:"s \<sim>. d .\<sim> t"
+        and   p2:"s' \<in> scheduleR sysconf s"
+        and   p3:"t' \<in> scheduleR sysconf t"
+      shows   "s' \<sim>. d .\<sim>\<^sub>\<Delta> t'" using p1 p2 p3 by auto
+
+
+  lemma scheduleR_presrv_wk_stp_cons_new_e: "weak_step_consistent_new_e (sys' Schedule)"
+    using scheduleR_presrv_wk_stp_cons_new weak_step_consistent_new_e_def 
+      exec_eventR_def same_part_mode sched_vpeq 
+          by (smt EventR.case(2) System_EventR.case(1) State.select_convs(1) State.select_convs(2) 
+                abstract_state_def domain_of_eventR_sys event_enabledR_sys mem_Collect_eq 
+                singletonD vpeqR_def option.sel prod.simps(2))
+
+  lemma trans_smpl_msgR_presrv_wk_stp_cons_new:
+      assumes 
+              p1:"s \<sim>. d .\<sim> t"
+        and   p2:"s' = transf_sampling_msgR s c"
+        and   p3:"t' = transf_sampling_msgR t c"
+      shows   "s' \<sim>. d .\<sim>\<^sub>\<Delta> t'" using p1 p2 p3 by auto
+    
+
+  lemma trans_smpl_msgR_presrv_wk_stp_cons_new_e: "weak_step_consistent_new_e (sys' (Transfer_Sampling_Message c))"
+    using trans_smpl_msgR_presrv_wk_stp_cons_new weak_step_consistent_new_e_def 
+      exec_eventR_def same_part_mode is_a_transmitter_def vpeq1_def vpeq_sched_def
+          by (smt EventR.case(2) System_EventR.case(2) State.select_convs(1) State.select_convs(2) 
+                abstract_state_def domain_of_eventR_sys event_enabledR_sys mem_Collect_eq 
+                singletonD vpeqR_def option.sel prod.simps(2))
+
+  lemma trans_que_msg_mlostR_presrv_wk_stp_cons_new:
+      assumes p1:"s \<sim>. d .\<sim> t"
+        and   p2:"s' = transf_queuing_msg_maylostR sysconf s c"
+        and   p3:"t' = transf_queuing_msg_maylostR sysconf t c"
+      shows   "s' \<sim>. d .\<sim>\<^sub>\<Delta> t'" using p1 p2 p3 by auto
+
+  lemma trans_que_msg_mlostR_presrv_wk_stp_cons_new_e: "weak_step_consistent_new_e (sys' (Transfer_Queuing_Message c))"
+    using trans_que_msg_mlostR_presrv_wk_stp_cons_new weak_step_consistent_new_e_def 
+      exec_eventR_def same_part_mode is_a_transmitter_def vpeq1_def vpeq_sched_def 
+          by (smt EventR.case(2) System_EventR.case(3) State.select_convs(1) State.select_convs(2) 
+                abstract_state_def domain_of_eventR_sys event_enabledR_sys mem_Collect_eq 
+                singletonD vpeqR_def option.sel prod.simps(2))
+
+  lemma set_procs_to_normal_presrv_wk_stp_cons_new:
+    assumes p1:"is_a_partition sysconf d"      
+      and   p2:"s \<sim>. d .\<sim> t"
+      and   p3:"s \<sim>. (scheduler sysconf) .\<sim> t"
+      and   p4:"s' = set_procs_to_normal s (current s)"
+      and   p5:"t' = set_procs_to_normal t (current t)"
+    shows   "s' \<sim>. d .\<sim>\<^sub>\<Delta> t'"  
+    proof -
+      from p1 p2 have a0: "(partitions s) d = (partitions t) d"         
+        using part_imp_not_sch part_imp_not_tras by force            
+      then show ?thesis using p1 p2 p3 p4 p5  by auto
+    qed
+
+
+  lemma remove_partition_resources_presrv_wk_stp_cons_new:
+    assumes p1:"is_a_partition sysconf d"
+      and   p2:"s \<sim>. d .\<sim> t"
+      and   p3:"s \<sim>. (scheduler sysconf) .\<sim> t"
+      and   p4:"s' = remove_partition_resources s (current s)"
+      and   p5:"t' = remove_partition_resources t (current t)"
+    shows   "s' \<sim>. d .\<sim>\<^sub>\<Delta> t'" 
+    proof -
+      from p1 p2 have a0: "(partitions s) d = (partitions t) d" 
+         using part_imp_not_sch part_imp_not_tras by force            
+       show ?thesis using p1 p2 p3  p4 p5 by auto      
+    qed
+
+  lemma set_part_modeR_presrv_wk_stp_cons_new:
+    assumes p1:"is_a_partition sysconf (current s)"
+      and   p2:"reachable0 s \<and> reachable0 t"
+      and   p3:"s \<sim>. d .\<sim> t"
+      and   p4:"s \<sim>. (scheduler sysconf) .\<sim> t"
+      and   p5:"(current s) \<leadsto> d"
+      and   p6:"s \<sim>. (current s) .\<sim> t"
+      and   p7:"s' = set_partition_modeR sysconf s m"
+      and   p8:"t' = set_partition_modeR sysconf t m"
+   shows   "s' \<sim>. d .\<sim>\<^sub>\<Delta> t'"
+   proof(cases "is_a_partition sysconf d")
+      assume a0:"is_a_partition sysconf d"
+      show ?thesis
+      proof(cases "current s = d")
+        assume b0: "current s = d"
+        with p3 a0 have b1: "(partitions s) d = (partitions t) d" 
+          using part_imp_not_sch part_imp_not_tras by force
+          thus ?thesis using p3 p1 a0 b0 p8 p2 p4 p6 p7 by auto        
+      next
+        assume b0: "current s \<noteq> d"
+        with p1 p2 p7 a0 have b1: "vpeq_part_procs s d s'"
+          by auto 
+        from p1 p2 p3 p8 a0 p4 b0 have b2: "vpeq_part_procs t d t'"
+          by auto 
+        from p3 b1 a0 b2 show ?thesis by auto
+      qed
+  next
+    assume b1:"\<not> is_a_partition sysconf d"
+    show ?thesis using b1 by auto
+  qed
+            
+  lemma set_part_modeR_presrv_wk_stp_cons_new_e: "weak_step_consistent_new_e (hyperc' (Set_Partition_Mode p))"
+    using set_part_modeR_presrv_wk_stp_cons_new weak_step_consistent_new_e_def 
+      exec_eventR_def same_part_mode sched_vpeq singletonD EventR.case(1) Hypercall'.case(12)
+          by (smt State.select_convs(1) State.select_convs(2) 
+                abstract_state_def domain_of_eventR_hc event_enabledR_hc mem_Collect_eq 
+                singletonD vpeqR_def option.sel prod.simps(2))
+
+
+subsection{* New events preserve "step consistent" on new state variables *} 
+subsubsection{*proving "Create process"*}
+  lemma create_process_presrv_wk_stp_cons_new:
+      assumes p1:"is_a_partition sysconf (current s)"        
+        and   p2:"s \<sim>. d .\<sim> t"
+        and   p3:"s \<sim>. (scheduler sysconf) .\<sim> t"        
+        and   p4:"s \<sim>. (current s) .\<sim> t"
+        and   p5:"s' = fst (create_process s pri)"
+        and   p6:"t' = fst (create_process t pri)"
+      shows   "s' \<sim>. d .\<sim>\<^sub>\<Delta> t'"
+      proof(cases "is_a_partition sysconf d")
+        assume a0:"is_a_partition sysconf d"
+        from p3 have a1: "current s = current t" by auto
+        show ?thesis 
+          proof(cases "current s = d")
+            assume b0: "current s = d"
+            with p2 a0 have b1: "(partitions s) d = (partitions t) d" 
+              using part_imp_not_sch part_imp_not_tras by force              
+              thus ?thesis using p1  p2 p3 p4  p6 p5 by fastforce             
+          next
+            assume b0: "current s \<noteq> d"
+            with p5 have b1: "vpeq_part_procs s d s'" 
+              using create_process_vpeq_part_procs[OF b0 p5] by (simp cong del: )
+            moreover from p6 a0 a1 b0 have b2: "vpeq_part_procs t d t'"
+              using create_process_vpeq_part_procs[OF b0] by simp
+            ultimately  show ?thesis using p2  by auto 
+          qed
+      next
+        assume b1:"\<not> is_a_partition sysconf d"
+        then show ?thesis by auto
+      qed
+
+  lemma create_process_presrv_wk_stp_cons_new_e: "weak_step_consistent_new_e (hyperc' (Create_Process p))"
+    using create_process_presrv_wk_stp_cons_new weak_step_consistent_new_e_def exec_eventR_def 
+       same_part_mode sched_vpeq
+          by (smt EventR.case(1) Hypercall'.case(14) State.select_convs(1) State.select_convs(2) 
+                abstract_state_def domain_of_eventR_hc event_enabledR_hc mem_Collect_eq 
+                singletonD vpeqR_def option.sel prod.simps(2))
+
+
+subsubsection{*proving "set process priority"*}
+  lemma set_process_priority_presrv_wk_stp_cons_new:
+      assumes p1:"is_a_partition sysconf (current s)"
+        and   p2:"reachable0 s \<and> reachable0 t"
+        and   p3:"s \<sim>. d .\<sim> t"
+        and   p4:"s \<sim>. (scheduler sysconf) .\<sim> t"
+        and   p5:"s \<sim>. (current s) .\<sim> t"
+        and   p6:"s' = set_process_priority s pr pri"
+        and   p7:"t' = set_process_priority t pr pri"
+      shows   "s' \<sim>. d .\<sim>\<^sub>\<Delta> t'"
+      proof(cases "is_a_partition sysconf d")
+        assume a0:"is_a_partition sysconf d"
+        from p3 p4 have a1: "current s = current t" 
+          by auto
+        show ?thesis
+          proof(cases "current s = d")
+            assume b0: "current s = d"
+            with p3 a0 have b1: "(partitions s) d = (partitions t) d" 
+              using part_imp_not_sch part_imp_not_tras by force       
+            thus ?thesis using  p1 a0 b0 p5  p4 p6 p7 by auto
+          next
+            assume b0: "current s \<noteq> d"
+            with p1 p2 p6 a0 have b1: "vpeq_part_procs s d s'" 
+              by auto
+            from p1 p2 p7 a0 a1 b0 have b2: "vpeq_part_procs t d t'"
+              by auto
+            from p3 b1 a0 b2 show ?thesis by auto
+          qed
+      next
+        assume b1:"\<not> is_a_partition sysconf d"
+        then show ?thesis by auto
+      qed
+
+  lemma set_process_priority_presrv_wk_stp_cons_new_e: "weak_step_consistent_new_e (hyperc' (Set_Priority p pri))"
+    using set_process_priority_presrv_wk_stp_cons_new weak_step_consistent_new_e_def 
+      exec_eventR_def same_part_mode sched_vpeq domain_of_eventR_hc event_enabledR_hc 
+          by (smt EventR.case(1) Hypercall'.case(19) State.select_convs(1) State.select_convs(2) 
+                abstract_state_def mem_Collect_eq old.prod.case singletonD vpeqR_def option.sel prod.simps(2))
+
+subsubsection{*proving "start process"*}
+  lemma start_process_presrv_wk_stp_cons_new:
+      assumes p1:"is_a_partition sysconf (current s)"
+        and   p2:"reachable0 s \<and> reachable0 t"
+        and   p3:"s \<sim>. d .\<sim> t"
+        and   p4:"s \<sim>. (scheduler sysconf) .\<sim> t"       
+        and   p5:"s \<sim>. (current s) .\<sim> t"
+        and   p6:"s' = start_process s pr"
+        and   p7:"t' = start_process t pr"
+      shows   "s' \<sim>. d .\<sim>\<^sub>\<Delta> t'" 
+ proof(cases "is_a_partition sysconf d")
+      assume a0:"is_a_partition sysconf d"
+      from p3 p4 have a1: "current s = current t" 
+        by auto
+      show ?thesis
+        proof(cases "current s = d")
+          assume b0: "current s = d"
+          with p3 a0 have b1: "(partitions s) d = (partitions t) d" 
+            using part_imp_not_sch part_imp_not_tras by force       
+          thus ?thesis using  p1 a0 b0 p5  p4 p6 p7 by auto
+        next
+          assume b0: "current s \<noteq> d"
+          with p1 p2 p6 a0 have b1: "vpeq_part_procs s d s'" 
+            by auto
+          from p1 p2 p7 a0 a1 b0 have b2: "vpeq_part_procs t d t'"
+            by auto
+          from p3 b1 a0 b2 show ?thesis by auto
+        qed
+    next
+      assume b1:"\<not> is_a_partition sysconf d"
+      then show ?thesis by auto
+    qed
+     
+
+  lemma start_process_presrv_wk_stp_cons_new_e: "weak_step_consistent_new_e (hyperc' (Start_Process p))"
+    using start_process_presrv_wk_stp_cons_new weak_step_consistent_new_e_def 
+      exec_eventR_def same_part_mode sched_vpeq
+          by (smt EventR.case(1) Hypercall'.case(15) State.select_convs(1) State.select_convs(2) 
+                abstract_state_def domain_of_eventR_hc event_enabledR_hc mem_Collect_eq 
+                singletonD vpeqR_def option.sel prod.simps(2))
+
+subsubsection{*proving "stop process"*}
+  lemma stop_process_presrv_wk_stp_cons_new:
+  assumes p1:"is_a_partition sysconf (current s)"
+    and   p2:"reachable0 s \<and> reachable0 t"
+    and   p3:"s \<sim>. d .\<sim> t"
+    and   p4:"s \<sim>. (scheduler sysconf) .\<sim> t"
+    and   p5:"s \<sim>. (current s) .\<sim> t"
+    and   p6:"s' = stop_process s pr"
+    and   p7:"t' = stop_process t pr"
+  shows   "s' \<sim>. d .\<sim>\<^sub>\<Delta> t'"
+  using p1 p2 p3 p4 p5 p6 p7 by auto
+  
+  lemma stop_process_presrv_wk_stp_cons_new_e: "weak_step_consistent_new_e (hyperc' (Stop_Process p))"
+    using stop_process_presrv_wk_stp_cons_new weak_step_consistent_new_e_def 
+      exec_eventR_def same_part_mode sched_vpeq
+          by (smt EventR.case(1) Hypercall'.case(16) State.select_convs(1) State.select_convs(2) 
+                abstract_state_def domain_of_eventR_hc event_enabledR_hc mem_Collect_eq 
+                singletonD vpeqR_def option.sel prod.simps(2))
+
+subsubsection{*proving "suspend process"*}
+  lemma suspend_process_presrv_wk_stp_cons_new:
+    assumes p1:"is_a_partition sysconf (current s)"
+      and   p2:"reachable0 s \<and> reachable0 t"
+      and   p3:"s \<sim>. d .\<sim> t"
+      and   p4:"s \<sim>. (scheduler sysconf) .\<sim> t"     
+      and   p5:"s \<sim>. (current s) .\<sim> t"
+      and   p6:"s' = suspend_process s pr"
+      and   p7:"t' = suspend_process t pr"
+    shows   "s' \<sim>. d .\<sim>\<^sub>\<Delta> t'"
+using p1 p2 p3 p4 p5 p6 p7 by auto
+
+  lemma suspend_process_presrv_wk_stp_cons_new_e: "weak_step_consistent_new_e (hyperc' (Suspend_Process p))"
+    using suspend_process_presrv_wk_stp_cons_new weak_step_consistent_new_e_def 
+      exec_eventR_def same_part_mode sched_vpeq
+          by (smt EventR.case(1) Hypercall'.case(18) State.select_convs(1) State.select_convs(2) 
+                abstract_state_def domain_of_eventR_hc event_enabledR_hc mem_Collect_eq 
+                singletonD vpeqR_def option.sel prod.simps(2))
+
+subsubsection{*proving "resume process"*}
+  lemma resume_process_presrv_wk_stp_cons_new:
+  assumes p1:"is_a_partition sysconf (current s)"
+    and   p2:"reachable0 s \<and> reachable0 t"
+    and   p3:"s \<sim>. d .\<sim> t"
+    and   p4:"s \<sim>. (scheduler sysconf) .\<sim> t"
+    and   p5:"s \<sim>. (current s) .\<sim> t"
+    and   p6:"s' = resume_process s pr"
+    and   p7:"t' = resume_process t pr"
+  shows   "s' \<sim>. d .\<sim>\<^sub>\<Delta> t'"
+  using p1 p2 p3 p4 p5 p6 p7 by auto
+
+  lemma resume_process_presrv_wk_stp_cons_new_e: "weak_step_consistent_new_e (hyperc' (Resume_Process p))"
+    using resume_process_presrv_wk_stp_cons_new weak_step_consistent_new_e_def 
+      exec_eventR_def same_part_mode sched_vpeq
+          by (smt EventR.case(1) Hypercall'.case(17) State.select_convs(1) State.select_convs(2) 
+                abstract_state_def domain_of_eventR_hc event_enabledR_hc mem_Collect_eq 
+                singletonD vpeqR_def option.sel prod.simps(2))
+
+subsubsection{*proving "get process status"*}
+  lemma get_process_status_presrv_wk_stp_cons_new:
+      assumes p1:"s \<sim>. d .\<sim> t"
+        and   p2:"s' = fst (get_process_status s pr)"
+        and   p3:"t' = fst (get_process_status t pr)"
+      shows   "s' \<sim>. d .\<sim>\<^sub>\<Delta> t'"
+    proof -
+      have a0:"s' = s" using p2 by auto 
+      have a1:"t' = t" using p3 by auto 
+      then show ?thesis using a0 p1 by auto
+    qed
+
+  lemma get_process_status_presrv_wk_stp_cons_new_e: "weak_step_consistent_new_e (hyperc' (Get_Process_Status p))"
+    using get_process_status_presrv_wk_stp_cons_new weak_step_consistent_new_e_def 
+      exec_eventR_def domain_of_eventR_def event_enabledR_def same_part_mode sched_vpeq 
+      non_interference1_def non_interference_def singletonD 
+          by (smt EventR.case(1) Hypercall'.case(20) State.select_convs(1) State.select_convs(2) 
+                abstract_state_def domain_of_eventR_hc event_enabledR_hc mem_Collect_eq 
+                singletonD vpeqR_def option.sel prod.simps(2))
+
+subsubsection{*proving "schedule process"*}
+  lemma setrun2ready_presrv_wk_stp_cons_new:
+      assumes 
+              p1:"s \<sim>. d .\<sim> t"
+        and   p2:"s \<sim>. (scheduler sysconf) .\<sim> t"        
+        and   p3:"s' = setRun2Ready s"
+        and   p4:"t' = setRun2Ready t"
+      shows   "s' \<sim>. d .\<sim>\<^sub>\<Delta> t'"
+     using  p1 p2 p3 p4 by auto
+
+  lemma schedule_process_presrv_wk_stp_cons_new:
+    assumes p1:"is_a_partition sysconf (current s)"
+      and   p2:"reachable0 s \<and> reachable0 t"
+      and   p3:"s \<sim>. d .\<sim> t"
+      and   p4:"s \<sim>. (scheduler sysconf) .\<sim> t"
+      and   p5:"(current s) \<leadsto> d"
+      and   p6:"s \<sim>. (current s) .\<sim> t"
+      and   p7:"s' \<in> schedule_process s"
+      and   p8:"t' \<in> schedule_process t"
+    shows   "s' \<sim>. d .\<sim>\<^sub>\<Delta> t'"
+   
+    proof(cases "is_a_partition sysconf d")
+      assume a0:"is_a_partition sysconf d"
+      from p3 p4 have a1: "current s = current t" 
+        using sched_currentR_lemma domain_of_eventR_hc
+          by auto
+      show ?thesis
+      proof(cases "current s = d")
+        assume b0: "current s = d"
+        with p3 a0 have b1: "(partitions s) d = (partitions t) d" 
+          using part_imp_not_sch part_imp_not_tras by force 
+        from p3 a0 have b2: "vpeq_part_procs s d t" by (simp add: vpeqR_def)
+        with p1 b0 have b3: "(procs s) d = (procs t) d \<and>
+                       (\<forall>p. (proc_state s) (d,p) = (proc_state t) (d,p))\<and>
+                       (cur_proc_part s) d = (cur_proc_part t) d" 
+          by auto
+        with p7 p8 have r1: "procs s' d = procs t' d" 
+          using schedule_process_def setRun2Ready_def by (smt StateR.select_convs(1) StateR.surjective 
+            StateR.update_convs(2) StateR.update_convs(3)  singletonD) 
+        moreover
+        have r2: "(cur_proc_part s') d = (cur_proc_part t') d \<and> (\<forall>p. (proc_state s') (d,p) = (proc_state t') (d,p))"
+        proof -
+          let ?cons = "is_a_partition sysconf (current s) 
+                    \<and> part_mode (the ((partitions s) (current s))) = NORMAL"
+          let ?cont = "is_a_partition sysconf (current t) 
+                    \<and> part_mode (the ((partitions t) (current t))) = NORMAL"
+          have b9: "?cons = ?cont" using a1 b0 b1 by auto 
+          show ?thesis 
+          proof(cases "?cons")
+            assume c0: "?cons"            
+            then have c1: "?cont" using b9 by simp
+            let ?s' = "setRun2Ready s"
+            let ?readyprs = "{p. p\<in>the (procs ?s' (current ?s')) \<and> 
+                                    state (the (proc_state ?s' (current ?s',p))) = READY}"
+            let ?selp = "SOME p. p\<in>{x. state (the (proc_state ?s' (current ?s',x))) = READY \<and>
+                                                   (\<forall>y\<in>?readyprs. priority (the (proc_state ?s' (current ?s',x))) \<ge>
+                                                                priority (the (proc_state ?s' (current ?s',y))))}"
+            let ?st = "the ((proc_state ?s') (current ?s', ?selp))"
+            let ?proc_st = "proc_state ?s'"
+            let ?cur_pr = "cur_proc_part ?s'"
+            from c0 have c2: "schedule_process s = {?s'\<lparr>proc_state := ?proc_st ((current ?s', ?selp) := Some (?st\<lparr>state := RUNNING\<rparr>)),
+                                             cur_proc_part := ?cur_pr(current ?s' := Some ?selp)\<rparr>}"
+              using schedule_process_def [of s] by auto
+            
+            let ?t' = "setRun2Ready t"
+            let ?readyprst = "{p. p\<in>the (procs ?t' (current ?t')) \<and> 
+                                    state (the (proc_state ?t' (current ?t',p))) = READY}"
+            let ?selpt = "SOME p. p\<in>{x. state (the (proc_state ?t' (current ?t',x))) = READY \<and>
+                                                     (\<forall>y\<in>?readyprst. priority (the (proc_state ?t' (current ?t',x))) \<ge>
+                                                                  priority (the (proc_state ?t' (current ?t',y))))}"
+            let ?stt = "the ((proc_state ?t') (current ?t', ?selpt))"
+            let ?proc_stt = "proc_state ?t'"
+            let ?cur_prt = "cur_proc_part ?t'"
+            from c1 have c3: "schedule_process t = {?t'\<lparr>proc_state := ?proc_stt ((current ?t', ?selpt) := Some (?stt\<lparr>state := RUNNING\<rparr>)),
+                                             cur_proc_part := ?cur_prt(current ?t' := Some ?selpt)\<rparr>}"
+              using schedule_process_def [of t] by auto
+            have c4: "?s' \<sim>. d .\<sim>\<^sub>\<Delta> ?t'"
+              using b0 p1 p2 p4 p6 setrun2ready_presrv_wk_stp_cons_new 
+              by (fastforce cong del:setRun2Ready_def vpeq_part_procs_def)
+            then have c5: "((procs ?s') d = (procs ?t') d) \<and>
+                        (\<forall>p. (proc_state ?s') (d,p) = (proc_state ?t') (d,p)) \<and>
+                        (cur_proc_part ?s') d = (cur_proc_part ?t') d"
+              using a0 by auto                         
+            have c7: "current ?s' = current ?t'" using a1 
+              by fastforce 
+            have c8: "current s = current ?s'" using a1 setrun2ready_nchastate_lemma by fastforce                                                             
+            then  show ?thesis using  p7 p8 c2 a0 c3 c5 a0 c7 c8 b0 a1 
+             by (fastforce cong del: setRun2Ready_def)
+          next
+            assume c0: "\<not> ?cons"
+            thus ?thesis using p7 p8 p3 b3 b9 by auto 
+          qed        
+        qed
+        ultimately show ?thesis
+          by auto
+      next
+        assume b0: "current s \<noteq> d"                        
+        from  p8 p7 a0 a1 b0 p3   
+        show ?thesis using schedule_process_vpeq_part_procs
+          by (auto cong del: setRun2Ready_def)
+      qed
+    next
+      assume b1:"\<not> is_a_partition sysconf d"
+      then show ?thesis by auto
+    qed
+
+  lemma schedule_process_presrv_wk_stp_cons_new_e: "weak_step_consistent_new_e (sys' Schedule_Process)"
+    using schedule_process_presrv_wk_stp_cons_new weak_step_consistent_new_e_def 
+      exec_eventR_def same_part_mode sched_vpeq 
+          by (smt EventR.case(2) System_EventR.case(4) State.select_convs(1) State.select_convs(2) 
+                abstract_state_def domain_of_eventR_sys event_enabledR_sys mem_Collect_eq 
+                singletonD vpeqR_def option.sel prod.simps(2))
+
+subsection{* Proving the "step consistent" property on new state variables *}
+  theorem weak_step_consistent_new:weak_step_consistent_new
+    proof -
+      {
+        fix e
+        have "weak_step_consistent_new_e e"
+          apply(induct e)
+          using crt_smpl_portR_presrv_wk_stp_cons_new_e wrt_smpl_msgR_presrv_wk_stp_cons_new_e 
+                 read_smpl_msgR_presrv_wk_stp_cons_new_e get_smpl_pidR_presrv_wk_stp_cons_new_e
+                 get_smpl_pstsR_presrv_wk_stp_cons_new_e crt_que_portR_presrv_wk_stp_cons_new_e 
+                 snd_que_msg_lstR_presrv_wk_stp_cons_new_e rec_que_msgR_presrv_wk_stp_cons_new_e 
+                 get_que_pidR_presrv_wk_stp_cons_new_e get_que_pstsR_presrv_wk_stp_cons_new_e
+                 clr_que_portR_presrv_wk_stp_cons_new_e set_part_modeR_presrv_wk_stp_cons_new_e 
+                 get_part_statusR_presrv_wk_stp_cons_new_e create_process_presrv_wk_stp_cons_new_e 
+                 start_process_presrv_wk_stp_cons_new_e stop_process_presrv_wk_stp_cons_new_e
+                 resume_process_presrv_wk_stp_cons_new_e suspend_process_presrv_wk_stp_cons_new_e 
+                 set_process_priority_presrv_wk_stp_cons_new_e get_process_status_presrv_wk_stp_cons_new_e 
+          apply(rule Hypercall'.induct)
+          using scheduleR_presrv_wk_stp_cons_new_e trans_smpl_msgR_presrv_wk_stp_cons_new_e
+              trans_que_msg_mlostR_presrv_wk_stp_cons_new_e schedule_process_presrv_wk_stp_cons_new_e
+              by (rule System_EventR.induct)
+      }
+      then show ?thesis using weak_step_consistent_new_all_evt by simp
+    qed
+
+subsection{* Information flow security of second-level specification *}
+  theorem noninfluence_sat: noninfluence
+    using noninfl_refinement local_respect_new weak_step_consistent_new
+      local_respect weak_step_consistent by blast
+
+  theorem noninfluence_gen_sat: noninfluence_gen
+    using noninf_eq_noninf_gen noninfluence_sat by blast 
+
+  theorem weak_noninfluence_sat: weak_noninfluence
+    using noninf_impl_weak noninfluence_sat by blast
+    
+  theorem nonleakage_sat: nonleakage
+    using noninf_impl_nonlk noninfluence_sat by blast
+  
+  theorem noninterference_r_sat: noninterference_r
+    using noninf_impl_nonintf_r noninfluence_sat by blast
+    
+  theorem noninterference_sat: noninterference
+    using noninterference_r_sat nonintf_r_impl_noninterf by blast
+    
+  theorem weak_noninterference_r_sat: weak_noninterference_r
+    using noninterference_r_sat nonintf_r_impl_wk_nonintf_r by blast
+    
+  theorem weak_noninterference_sat: weak_noninterference
+    using noninterference_sat nonintf_impl_weak by blast
+
+end
